cheririscV/Asm.v
@@ -17,7 +17,7 @@
 
 (** Abstract syntax and semantics for RISC-V assembly language. *)
 
-Require Import Coqlib.
+Require Import Coqlib List.
 Require Import Maps.
 Require Import CapAST.
 Require Import Integers.
@@ -25,13 +25,15 @@ Require Import Floats.
 Require Import OCapValues.
 Require Import CapMemory.
 Require Import Events.
-Require Import Globalenvs.
+Require Import CapGlobalenvs.
 Require Import Smallstep.
-Require Import Locations.
+Require Import CapLocations.
 Require Stacklayout.
 Require Import Conventions.
 
 Notation offset_arg := Stacklayout.offset_arg.
+
+Local Open Scope error_monad_scope.
 
 (** * Abstract syntax *)
 
@@ -48,7 +50,7 @@ Inductive ireg: Type :=
   | X16: ireg | X17: ireg | X18: ireg | X19: ireg | X20: ireg
   | X21: ireg | X22: ireg | X23: ireg | X24: ireg | X25: ireg
   | X26: ireg | X27: ireg | X28: ireg | X29: ireg | X30: ireg
-  | X31: ireg.
+  | X31: ireg | X32 : ireg.
 
 Inductive ireg0: Type :=
   | X0: ireg0 | X: ireg -> ireg0.
@@ -88,12 +90,27 @@ Proof. decide equality. Defined.
 
  *)
 
+(** registers that can contain capabilities *)
+Inductive creg: Type :=
+  | IRcap: ireg -> creg
+  | PCcap: creg
+  | DDcap: creg.
+
 Inductive preg: Type :=
   | IR: ireg -> preg                    (**r integer registers *)
   | FR: freg -> preg                    (**r double-precision float registers *)
   | PCC: preg                          (**r program counter capability *)
   | DDC: preg.                         (**r default data capability *) 
 
+Definition creg_to_preg (c: creg) : preg :=
+  match c with
+  | IRcap i => IR i
+  | PCcap => PCC
+  | DDcap => DDC
+  end.
+
+Coercion creg_to_preg: creg >-> preg.
+Coercion IRcap: ireg >-> creg.
 Coercion IR: ireg >-> preg.
 Coercion FR: freg >-> preg.
 
@@ -109,13 +126,14 @@ Module Pregmap := EMap(PregEq).
 
 (** Conventional names for stack pointer ([SPC]) and return address code and data ([RAC] & [RAD]). *)
 
-(** Each with hold capabilities: an uninitialized directed capability
+(** Each will hold capabilities: an uninitialized directed capability
     in SPC and a sealed return & data capability pair in RAC and RAD
 *)
 
 Notation "'SPC'" := X3 (only parsing) : asm.
 Notation "'RAC'" := X1 (only parsing) : asm.
-Notation "'RAD'" := X2 (only parsing) : asm.
+Notation "'SPPC'" := X2 (only parsing) : asm.
+Notation "'EC'" := X31 (only parsing) : asm.
 
 (** Offsets for load and store instructions.  An offset is either an
   immediate integer or the low part of a symbol. *)
@@ -213,7 +231,10 @@ Definition label := positive.
   [Asmgen]) is careful to respect this range. *)
 
 Inductive instruction : Type :=
-  | Pmv     (rd: ireg) (rs: ireg)                    (**r integer move *)
+  | Pmv     (rd: creg) (rs: creg)                    (**r integer or capability move, 
+                                                        includes from a special purpose 
+                                                        capability register 
+                                                        ([CReadHwr] and [CWriteHwr] in CHERI) *)
 
 (** 32-bit integer register-immediate instructions *)
   | Paddiw  (rd: ireg) (rs: ireg0) (imm: int)        (**r add immediate *)
@@ -289,13 +310,13 @@ Inductive instruction : Type :=
      Branches to labels or symbols indirectly use the PCC. *)
             
   (* Unconditional jumps.  Links are always to X1/RA. *)
-  | Pj_l    (l: label)                              (**r jump to label *)
-  | Pj_s    (symb: ident) (sg: signature)           (**r jump to symbol *)
-  | Pj_r    (r: ireg)     (sg: signature) (iscl: bool) (**r jump register *)
-  | Pjal_s  (symb: ident) (sg: signature) (iscl: bool) (**r jump-and-link symbol *)
-  | Pjal_r  (r: ireg)     (sg: signature) (iscl: bool) (**r jump-and-link register *)
-  | PCjal_r (rs1 rs2: ireg) (sg: signature) (iscl: bool) (**r jump-and-link capability
-                                                         jumps to rs2, seals the next PCC as in rs1 *)
+  | Pj_l    (l: label)                                        (**r jump to label *)
+  (* | Pj_s    (symb: ident)           (sg: signature)           (**r jump to symbol *) *)
+  | Pj_r    (r: ireg)               (* (sg: signature) (iscl: bool) jump is no longer a return event marker *) (**r jump register *)
+  (* | Pjal_s  (symb: ident)           (sg: signature) (iscl: bool) (**r jump-and-link symbol *) *)
+  | Pjal_r  (r: ireg)               (sg: signature) (iscl: bool) (**r jump-and-link register *)
+  (* | PCjal_s (symb: ident) (s: ireg) (sg: signature) (iscl: bool) (**r jump-and-sealed-link symbol *) *)
+  | PCjal_r (r s: ireg)             (sg: signature) (iscl: bool) (**r jump-and-sealed-link register *)
             
   (* Conditional branches, 32-bit comparisons *)
   | Pbeqw   (rs1 rs2: ireg0) (l: label)             (**r branch-if-equal *)
@@ -314,9 +335,9 @@ Inductive instruction : Type :=
   | Pbgeul  (rs1 rs2: ireg0) (l: label)             (**r branch-if-greater-or-equal unsigned *)
 
   (* Sealed capability invocation *)
-  | PCinvoke (rs1 rs2: ireg0)                        (**r unseal and jump to rs2 while unsealing rs1 *)
+  | PCinvoke (rs1 rs2: ireg0) (iscl: bool)             (**r unseal and jump to rs2 while unsealing rs1 *)
 
-  (* Legacy loads and stores: semantics use the DDC *)
+  (* Legacy loads and stores: semantics use the DDC: ireg is expected to hold a heap pointer (integer) *)
   | Plb     (rd: ireg) (ra: ireg) (ofs: offset) (priv: bool)    (**r load signed int8 *)
   | Plbu    (rd: ireg) (ra: ireg) (ofs: offset) (priv: bool)    (**r load unsigned int8 *)
   | Plh     (rd: ireg) (ra: ireg) (ofs: offset) (priv: bool)    (**r load signed int16 *)
@@ -335,58 +356,110 @@ Inductive instruction : Type :=
   | Psw_a   (rs: ireg) (ra: ireg) (ofs: offset)     (**r store any32 *)
   | Psd     (rs: ireg) (ra: ireg) (ofs: offset)     (**r store int64 *)
   | Psd_a   (rs: ireg) (ra: ireg) (ofs: offset)     (**r store any64 *)
+  | Pscw    (rs: ireg) (ra: ireg) (ofs: offset)     (**r store cap64 *)
+  | Pscd    (rs: ireg) (ra: ireg) (ofs: offset)     (**r store cap128 *)
+  | Pscd_a  (rs: ireg) (ra: ireg) (ofs: offset)     (**r store any128 *)
 
-  (* Capability load and stores: ra is expected to hold an unsealed capability *)
-  | PClb    (rd: ireg) (ra: ireg) (ofs: offset) (priv: bool)    (**r load signed int8 *)
-  | PClbu   (rd: ireg) (ra: ireg) (ofs: offset) (priv: bool)    (**r load unsigned int8 *)
-  | PClh    (rd: ireg) (ra: ireg) (ofs: offset) (priv: bool)    (**r load signed int16 *)
-  | PClhu   (rd: ireg) (ra: ireg) (ofs: offset) (priv: bool)    (**r load unsigned int16 *)
-  | PClw    (rd: ireg) (ra: ireg) (ofs: offset) (priv: bool)    (**r load int32 *)
-  | PClw_a  (rd: ireg) (ra: ireg) (ofs: offset) (priv: bool)    (**r load any32 *)
-  | PCld    (rd: ireg) (ra: ireg) (ofs: offset) (priv: bool)    (**r load int64 *)
-  | PCld_a  (rd: ireg) (ra: ireg) (ofs: offset) (priv: bool)    (**r load any64 *)
-  | PClwc   (rd: ireg) (ra: ireg) (ofs: offset) (priv: bool)    (**r load cap64 *)
-  | PClcd   (rd: ireg) (ra: ireg) (ofs: offset) (priv: bool)    (**r load cap128 *)
-  | PClcd_a (rd: ireg) (ra: ireg) (ofs: offset) (priv: bool)    (**r load any128 *)
+  (* Capability load and stores: ra is expected to hold an unsealed initialized capability *)
+  | PClb    (rd: ireg) (ra: ireg) (ofs: offset) (h priv: bool)    (**r load signed int8 *)
+  | PClbu   (rd: ireg) (ra: ireg) (ofs: offset) (h priv: bool)    (**r load unsigned int8 *)
+  | PClh    (rd: ireg) (ra: ireg) (ofs: offset) (h priv: bool)    (**r load signed int16 *)
+  | PClhu   (rd: ireg) (ra: ireg) (ofs: offset) (h priv: bool)    (**r load unsigned int16 *)
+  | PClw    (rd: ireg) (ra: ireg) (ofs: offset) (h priv: bool)    (**r load int32 *)
+  | PClw_a  (rd: ireg) (ra: ireg) (ofs: offset) (h priv: bool)    (**r load any32 *)
+  | PCld    (rd: ireg) (ra: ireg) (ofs: offset) (h priv: bool)    (**r load int64 *)
+  | PCld_a  (rd: ireg) (ra: ireg) (ofs: offset) (h priv: bool)    (**r load any64 *)
+  | PClwc   (rd: ireg) (ra: ireg) (ofs: offset) (h priv: bool)    (**r load cap64 *)
+  | PClcd   (rd: ireg) (ra: ireg) (ofs: offset) (h priv: bool)    (**r load cap128 *)
+  | PClcd_a (rd: ireg) (ra: ireg) (ofs: offset) (h priv: bool)    (**r load any128 *)
             
-  | PCsb    (rs: ireg) (ra: ireg) (ofs: offset)     (**r store int8 *)
-  | PCsh    (rs: ireg) (ra: ireg) (ofs: offset)     (**r store int16 *)
-  | PCsw    (rs: ireg) (ra: ireg) (ofs: offset)     (**r store int32 *)
-  | PCsw_a  (rs: ireg) (ra: ireg) (ofs: offset)     (**r store any32 *)
-  | PCsd    (rs: ireg) (ra: ireg) (ofs: offset)     (**r store int64 *)
-  | PCsd_a  (rs: ireg) (ra: ireg) (ofs: offset)     (**r store any64 *)
-  | PCscw   (rs: ireg) (ra: ireg) (ofs: offset)     (**r store cap64 *)
-  | PCscd   (rs: ireg) (ra: ireg) (ofs: offset)     (**r store cap128 *)
-  | PCscd_a (rs: ireg) (ra: ireg) (ofs: offset)     (**r store any128 *)
+  | PCsb    (rs: ireg) (ra: ireg) (ofs: offset) (h: bool)    (**r store int8 *)
+  | PCsh    (rs: ireg) (ra: ireg) (ofs: offset) (h: bool)    (**r store int16 *)
+  | PCsw    (rs: ireg) (ra: ireg) (ofs: offset) (h: bool)    (**r store int32 *)
+  | PCsw_a  (rs: ireg) (ra: ireg) (ofs: offset) (h: bool)    (**r store any32 *)
+  | PCsd    (rs: ireg) (ra: ireg) (ofs: offset) (h: bool)    (**r store int64 *)
+  | PCsd_a  (rs: ireg) (ra: ireg) (ofs: offset) (h: bool)    (**r store any64 *)
+  | PCscw   (rs: ireg) (ra: ireg) (ofs: offset) (h: bool)    (**r store cap64 *)
+  | PCscd   (rs: ireg) (ra: ireg) (ofs: offset) (h: bool)    (**r store cap128 *)
+  | PCscd_a (rs: ireg) (ra: ireg) (ofs: offset) (h: bool)    (**r store any128 *)
+
+  | PCfls     (rd: freg) (ra: ireg) (ofs: offset) (h priv: bool)    (**r load float *)
+  | PCfss     (rs: freg) (ra: ireg) (ofs: offset) (h: bool)         (**r store float *)
+  | PCfld     (rd: freg) (ra: ireg) (ofs: offset) (h priv: bool)    (**r load 64-bit float *)
+  | PCfld_a   (rd: freg) (ra: ireg) (ofs: offset) (h priv: bool)    (**r load any64 *)
+  | PCfsd     (rd: freg) (ra: ireg) (ofs: offset) (h: bool)         (**r store 64-bit float *)
+  | PCfsd_a   (rd: freg) (ra: ireg) (ofs: offset) (h: bool)         (**r store any64 *)
+            
+  (* Capability load and stores: ra is expected to hold an unsealed uninitialized capability *)
+  | PCUlb    (rd: ireg) (ra: ireg) (ro: ireg) (ofs: offset) (h priv: bool)    (**r load signed int8 *)
+  | PCUlbu   (rd: ireg) (ra: ireg) (ro: ireg) (ofs: offset) (h priv: bool)    (**r load unsigned int8 *)
+  | PCUlh    (rd: ireg) (ra: ireg) (ro: ireg) (ofs: offset) (h priv: bool)    (**r load signed int16 *)
+  | PCUlhu   (rd: ireg) (ra: ireg) (ro: ireg) (ofs: offset) (h priv: bool)    (**r load unsigned int16 *)
+  | PCUlw    (rd: ireg) (ra: ireg) (ro: ireg) (ofs: offset) (h priv: bool)    (**r load int32 *)
+  | PCUlw_a  (rd: ireg) (ra: ireg) (ro: ireg) (ofs: offset) (h priv: bool)    (**r load any32 *)
+  | PCUld    (rd: ireg) (ra: ireg) (ro: ireg) (ofs: offset) (h priv: bool)    (**r load int64 *)
+  | PCUld_a  (rd: ireg) (ra: ireg) (ro: ireg) (ofs: offset) (h priv: bool)    (**r load any64 *)
+  | PCUlwc   (rd: ireg) (ra: ireg) (ro: ireg) (ofs: offset) (h priv: bool)    (**r load cap64 *)
+  | PCUlcd   (rd: ireg) (ra: ireg) (ro: ireg) (ofs: offset) (h priv: bool)    (**r load cap128 *)
+  | PCUlcd_a (rd: ireg) (ra: ireg) (ro: ireg) (ofs: offset) (h priv: bool)    (**r load any128 *)
+            
+  | PCUsb    (rs: ireg) (ra: ireg) (ro: ireg) (ofs: offset) (h: bool)    (**r store int8 *)
+  | PCUsh    (rs: ireg) (ra: ireg) (ro: ireg) (ofs: offset) (h: bool)    (**r store int16 *)
+  | PCUsw    (rs: ireg) (ra: ireg) (ro: ireg) (ofs: offset) (h: bool)    (**r store int32 *)
+  | PCUsw_a  (rs: ireg) (ra: ireg) (ro: ireg) (ofs: offset) (h: bool)    (**r store any32 *)
+  | PCUsd    (rs: ireg) (ra: ireg) (ro: ireg) (ofs: offset) (h: bool)    (**r store int64 *)
+  | PCUsd_a  (rs: ireg) (ra: ireg) (ro: ireg) (ofs: offset) (h: bool)    (**r store any64 *)
+  | PCUscw   (rs: ireg) (ra: ireg) (ro: ireg) (ofs: offset) (h: bool)    (**r store cap64 *)
+  | PCUscd   (rs: ireg) (ra: ireg) (ro: ireg) (ofs: offset) (h: bool)    (**r store cap128 *)
+  | PCUscd_a (rs: ireg) (ra: ireg) (ro: ireg) (ofs: offset) (h: bool)    (**r store any128 *)
+             
+  | PCUfls     (rd: freg) (ra: ireg) (ro: ireg) (ofs: offset) (h priv: bool)    (**r load float *)
+  | PCUfss     (rs: freg) (ra: ireg) (ro: ireg) (ofs: offset) (h: bool)         (**r store float *)
+  | PCUfld     (rd: freg) (ra: ireg) (ro: ireg) (ofs: offset) (h priv: bool)    (**r load 64-bit float *)
+  | PCUfld_a   (rd: freg) (ra: ireg) (ro: ireg) (ofs: offset) (h priv: bool)    (**r load any64 *)
+  | PCUfsd     (rd: freg) (ra: ireg) (ro: ireg) (ofs: offset) (h: bool)         (**r store 64-bit float *)
+  | PCUfsd_a   (rd: freg) (ra: ireg) (ro: ireg) (ofs: offset) (h: bool)         (**r store any64 *)
 
   (* Capability-inspection instructions *)
   | PCgp    (rd: ireg) (ra: ireg)                   (**r get permission *)
   | PCgt    (rd: ireg) (ra: ireg)                   (**r get object type *)
-  | PCgb    (rd: ireg) (ra: ireg)                   (**r get base *)    
-  | PCge    (rd: ireg) (ra: ireg)                   (**r get end *)    
   | PCgg    (rd: ireg) (ra: ireg)                   (**r get tag *)    
   | PCgs    (rd: ireg) (ra: ireg)                   (**r get sealed status *)
-  | PCga    (rd: ireg) (ra: ireg)                   (**r get address offset *)
+  | PCga_s  (rd: ireg) (ra: ireg)                   (**r get address offset *)
+  | PCga_h  (rd: ireg) (ra: ireg)                   (**r get address offset *)
+  | PCgb_s  (rd: ireg) (ra: ireg)                   (**r get base *)    
+  | PCge_s  (rd: ireg) (ra: ireg)                   (**r get end *)    
+  | PCgb_h  (rd: ireg) (ra: ireg)                   (**r get base *)    
+  | PCge_h  (rd: ireg) (ra: ireg)                   (**r get end *)
+  | PCgl_s  (rd: ireg) (ra: ireg)                   (**r get length *)
+  | PCgl_h  (rd: ireg) (ra: ireg)                   (**r get length *)
 
   (* Capability-modification instructions *)          
   | PCseal      (rd: ireg) (rs1 rs2: ireg)             (**r sealing *)
   | PCunseal    (rd: ireg) (rs1 rs2: ireg)             (**r unsealing *)
-  | PCpermand   (rd: ireg) (rs1 rs2: ireg)             (**r bitwise and of permissions *)
-  | PCsaddr     (rd: ireg) (rs1 rs2: ireg)             (**r sets address of rs1 to rs2 *)
-  | PCiaddr     (rd: ireg) (rs1 rs2: ireg)             (**r increments address of rs1 by rs2 *)
-  | PCiaddr_il  (rd: ireg) (rs1 : ireg) (imm: int64)   (**r increments address of rs1 by imm *)
+  | PCpermand   (rd: ireg) (rs1 rs2: ireg)             (**r restricting the permission *)
+  | PCsaddr_w   (rd: ireg) (rs1 rs2: ireg)             (**r sets address of rs1 to rs2 *)
+  | PCsaddr_l   (rd: ireg) (rs1 rs2: ireg)             (**r sets address of rs1 to rs2 *)
+  | PCiaddr_w   (rd: ireg) (rs1 rs2: ireg0)            (**r increments address of rs1 by rs2 *)
+  | PCiaddr_l   (rd: ireg) (rs1 rs2: ireg0)            (**r increments address of rs1 by rs2 *)
+  | PCiaddr_iw  (rd: ireg) (rs1 : ireg0) (imm: int)    (**r increments address of rs1 by imm for 32 bit arch *)
+  | PCiaddr_il  (rd: ireg) (rs1 : ireg0) (imm: int64)  (**r increments address of rs1 by imm for 64 bit arch *)
   | PCsbase     (rd: ireg) (rs1 rs2: ireg)             (**r sets base to current address with length rs2 *)
-  | PCsbase_il  (rd: ireg) (rs1 : ireg) (imm: int64)   (**r sets base to current address with length imm *)
-  | PCcleart    (rd: ireg) (rs: ireg)                  (**r clears tag of capability in rs *)
-  | PCbuild     (rd: ireg) (rs1 rs2: ireg)             (**r derive capability from rs1 with fields from rs2 *)
+  | PCsbase_iw  (rd: ireg) (rs1 : ireg) (imm: int)     (**r sets base to current address with length imm for 32 bit arch*)
+  | PCsbase_il  (rd: ireg) (rs1 : ireg) (imm: int64)   (**r sets base to current address with length imm for 64 bit arch*)
+  (* | PCcleart    (rd: ireg) (rs: ireg)                  (**r clears tag of capability in rs *) *)
   | PCCseal     (rd: ireg) (rs1 rs2: ireg)             (**r conditional sealing *)
-  | PCseal_e    (rd: ireg) (rs : ireg)                 (**r seals to a sentry capability (E permission) *)
+  | PCseal_e    (rd: ireg) (rs: ireg)                  (**r seals to a sentry capability (E permission) *)
+  | PCpromote   (rd: ireg) (rs: ireg)                  (**r promotes an uninitialized capability to its initialized counterpart *)
 
   (* Capability pointer arithmetic instructions *)
-  | PCtoPtr  (rd: ireg) (rs1 rs2: ireg)             (**r rd is set to rs1.address - rs2.base *)
-  | PCsub    (rd: ireg) (rs1 rs2: ireg)             (**r rd is set to rs1.address - rs2.address *)
-  | PCmov    (rd: ireg) (rs: ireg)                  (**r rd is set to rs *)
-
+  | PCtoPtr_h  (rd: ireg) (rs1 rs2: ireg)             (**r rd is set to rs1.address - rs2.base *)
+  | PCsub_h    (rd: ireg) (rs1 rs2: ireg)             (**r rd is set to rs1.address - rs2.address *)
+  | PCtoPtr_s  (rd: ireg) (rs1 rs2: ireg)             (**r rd is set to rs1.address - rs2.base *)
+  | PCsub_s    (rd: ireg) (rs1 rs2: ireg)             (**r rd is set to rs1.address - rs2.address *)
+  | PCUtoPtr_h (rd: ireg) (rs1 rs2: ireg)             (**r rd is set to rs1.end - rs2.address *)
+  | PCUtoPtr_s (rd: ireg) (rs1 rs2: ireg)             (**r rd is set to rs1.end - rs2.address *)
+               
   (* Capability pointer comparison instructions *)
   | PCsubset (rd: ireg) (rs1 rs2: ireg)             (**r rd is set to 1 if rs2 was derived from rs1 *)
   | PCeex    (rd: ireg) (rs1 rs2: ireg)             (**r rd is set to 1 if the in memory representations of rs1 and rs2 are equal *)
@@ -394,8 +467,11 @@ Inductive instruction : Type :=
   (* fast register clearing instructions *)
   | PCCclear  (imm: int)                            (**r i'th iregister is cleared if bit i in imm is 1, 0'th bit refers to DDC *)
   | PCCclearf (imm: int)                            (**r i'th fregister is cleared if bit i in imm is 1 *)
-(* TODO: can i32 be represented as a bit vector? *)
 
+  (* tag-memory access instructions *)
+  | PCloadtag (dst: ireg) (rs1: ireg)               (**r rd is set to a bitstring with the tags of capabilities located 
+                                                       in rs1.address to rs1.address + CAPS_PER_CACHE_LINE (bit i == 1 <-> rs1) *)
+              
 (* Probably doesn't need privilged stores because can't write directly to parameters. Instead
    writing to a parameter writes to a /copy/ of the parameter *)
 
@@ -486,15 +562,17 @@ Inductive instruction : Type :=
   (* | Pallocframe (sz: Z) (pos: ptrofs)               (**r allocate new stack frame *) *)
   (* | Pfreeframe  (sz: Z) (pos: ptrofs)               (**r deallocate stack frame and restore previous frame *) *)
   | Plabel  (lbl: label)                            (**r define a code label *)
-  | Ploadsymbol (rd: ireg) (id: ident) (ofs: ptrofs) (**r load the address of a symbol *)
-  | Ploadsymbol_high (rd: ireg) (id: ident) (ofs: ptrofs) (**r load the high part of the address of a symbol *)
+  | Pptrbr  (rd: ireg) (lbl1 lbl2: label)           (**r branches to lbl1 if rd contains a heap ptr, lbl2 if rd contains a stack ptr *)
+  (* | Ploadsymbol (rd: ireg) (id: ident) (ofs: ptrofs) (**r load the address of a symbol *) *)
+  (* | Ploadsymbol_high (rd: ireg) (id: ident) (ofs: ptrofs) (**r load the high part of the address of a symbol *) *)
   | Ploadli (rd: ireg) (i: int64)                   (**r load an immediate int64 *)
   | Ploadfi (rd: freg) (f: float)                   (**r load an immediate float *)
   | Ploadsi (rd: freg) (f: float32)                 (**r load an immediate single *)
   | Pbtbl   (r: ireg)  (tbl: list label)            (**r N-way branch through a jump table *)
   | Pbuiltin: external_function -> list (builtin_arg preg)
               -> builtin_res preg -> instruction    (**r built-in function (pseudo) *)
-  | Pnop : instruction.                             (**r nop instruction *)
+  | Pnop : instruction                              (**r nop instruction *)
+  | Pfail : instruction.                            (**r fail instruction (deliberate crash) *)
 
 
 (** The pseudo-instructions are the following:
@@ -576,7 +654,7 @@ table:  .long   table[0], table[1], ...
     thus we do not need the stack related pseudo instructions *)
 
 Definition code := list instruction.
-Record function : Type := mkfunction { fn_comp: compartment; fn_sig: signature; fn_code: code }.
+Record function : Type := mkfunction { fn_comp: compartment; fn_sig: signature; fn_wrapper: code; fn_code: code }.
 Instance has_comp_function: has_comp function := fn_comp.
 Definition fundef := AST.fundef function.
 Definition program := AST.program fundef unit.
@@ -586,7 +664,7 @@ Definition program := AST.program fundef unit.
 (** The semantics operates over a single mapping from registers
   (type [preg]) to values.  We maintain
   the convention that integer registers are mapped to values of
-  type [Tint] or [Tlong] (in 64 bit mode),
+  type [Tcap], or [Tint] or [Tlong] (in 64 bit mode),
   and float registers to values of type [Tsingle] or [Tfloat]. *)
 
 Definition regset := Pregmap.t ocval.
@@ -635,6 +713,12 @@ Fixpoint set_regs (rl: list preg) (vl: list ocval) (rs: regset) : regset :=
   | _, _ => rs
   end.
 
+Fixpoint set_regs_default (rl: list preg) (v: ocval) (rs: regset) : regset :=
+  match rl with
+  | r1 :: rl' => set_regs_default rl' v (rs#r1 <- v)
+  | _ => rs
+  end.
+
 (** Assigning the result of a builtin *)
 
 Fixpoint set_res (res: builtin_res preg) (v: ocval) (rs: regset) : regset :=
@@ -679,6 +763,8 @@ Fixpoint label_pos (lbl: label) (pos: Z) (c: code) {struct c} : option Z :=
 
 Variable ge: genv.
 
+(* ALG: TODO: discuss below -> in a capability machine, the high part
+is specifically a capability *)
 (** The two functions below axiomatize how the linker processes
   symbolic references [symbol + offset)] and splits their
   actual values into a 20-bit high part [%hi(symbol + offset)] and 
@@ -693,7 +779,10 @@ Parameter high_half: genv -> ident -> ptrofs -> ocval.
 
 Axiom low_high_half:
   forall id ofs,
-  Val.offset_ptr (high_half ge id ofs) (low_half ge id ofs) = Some (Genv.symbol_address ge id ofs).
+    match Val.offset_ptr (high_half ge id ofs) (low_half ge id ofs) with
+    | Some ofs' => ofs' = (Genv.symbol_address ge id ofs)
+    | None => True
+    end.
 
 (** The semantics is purely small-step and defined as a function
   from the current state (a register set + a memory state)
@@ -703,21 +792,33 @@ Axiom low_high_half:
 
 Inductive outcome: Type :=
   | Next:  regset -> mem -> outcome
-  | Stuck: outcome.
+  | Stuck: outcome
+  | Crashed: outcome. (* we model capability failure as a crash *)
 
 (** Manipulations over the [PC] register: continuing with the next
   instruction ([nextinstr]) or branching to a label ([goto_label]). *)
 
-Definition nextinstr (rs: regset) :=
-  rs#PC <- (Val.offset_ptr rs#PC Ptrofs.one).
+Definition nextinstr (rs: regset) (m: mem) : outcome :=
+  match Val.offset_ptr rs#PCC Ptrofs.one with
+  | Some pc' => Next (rs#PCC <- pc') m
+  | None => Crashed
+  end.
 
+(* ALG: We do not model capability checks of the program
+counter. Thus, the address it points to is the relative offset within
+the program, rather than obsolute address *)
 Definition goto_label (f: function) (lbl: label) (rs: regset) (m: mem) :=
-  match label_pos lbl 0 (fn_code f) with
+  match label_pos lbl 0 (fn_wrapper f ++ fn_code f) with
   | None => Stuck
-  | Some pos =>
-      match rs#PC with
-      | Vptr b ofs => Next (rs#PC <- (Vptr b (Ptrofs.repr pos))) m
-      | _          => Stuck
+  | Some pos => (* pos is the relative offset *)
+      match rs#PCC with
+      | OCVcap (OCsealable (OCVmem RX Global b e a))
+                 => let a_lbl := Ptrofs.repr pos in (* a_lbl is the relative offset *)
+                   Next (rs#PCC <- (OCVcap (OCsealable (OCVmem RX Global b e a_lbl)))) m
+      | OCVcap (OCsealable (OCVmem RWX Global b e a))
+                 => let a_lbl := Ptrofs.repr pos in (* a_lbl is the relative offset *)
+                   Next (rs#PCC <- (OCVcap (OCsealable (OCVmem RX Global b e a_lbl)))) m
+      | _        => Crashed (* anything but an unsealed executable capability crashes *)
       end
   end.
 
@@ -729,20 +830,94 @@ Definition eval_offset (ofs: offset) : ptrofs :=
   | Ofslow id delta => low_half ge id delta
   end.
 
-Definition exec_load (chunk: memory_chunk) (rs: regset) (m: mem)
-                     (d: preg) (a: ireg) (ofs: offset) (cp: compartment) (priv: bool) :=
-  match Mem.loadv chunk m (Val.offset_ptr (rs a) (eval_offset ofs))
-                  (if priv then None else Some cp) with
-    | None => Stuck
-    | Some v => Next (nextinstr (rs#d <- v)) m
-    end.
+(* Definition eval_offset_val (rs: regset) (ofs: offset + ireg) (h: bool) : ocval := *)
+(*   match ofs with *)
+(*   | inl ofs' => if h then (OCVptr (heap_ptr (eval_offset ofs'))) *)
+(*                else (OCVptr (stack_ptr (eval_offset ofs'))) *)
+(*   | inr r => rs#r *)
+(*   end.       *)
 
+(* (* eval_act_kind detects if the givel value is an uninitialized *)
+(*   capability. By default the action kind is DIR *) *)
+(* Definition eval_act_kind (v: ocval) := *)
+(*   match v with *)
+(*   | OCVcap c => if isUCap c then UNINIT else DIR *)
+(*   | _ => DIR *)
+(*   end. *)
 
-Definition exec_store (chunk: memory_chunk) (rs: regset) (m: mem)
-                      (s: preg) (a: ireg) (ofs: offset) (cp: compartment) :=
-  match Mem.storev chunk m (Val.offset_ptr (rs a) (eval_offset ofs)) (rs s) cp with
+Definition zero_offset (h: bool) : ocval :=
+  if h then (OCVptr (heap_ptr Ptrofs.zero))
+  else (OCVptr (stack_ptr Ptrofs.zero)).
+
+Definition exec_load_capability (chunk: cap_memory_chunk) (rs: regset) (m: mem)
+           (d: preg) (a: ireg) (ofs: offset) (cp: compartment) (h priv: bool) :=
+  match Val.offset_ptr (rs a) (eval_offset ofs) with
+  | Some c => match Mem.loadv DIR chunk m c (zero_offset h)
+                             (if priv then None else Some cp) with
+             | inr PtrErr => Stuck
+             | inr CapErr => Crashed
+             | inl v => nextinstr (rs#d <- v) m
+             end
+  | _ => Stuck
+  end.
+
+Definition exec_load_Ucapability (chunk: cap_memory_chunk) (rs: regset) (m: mem)
+           (d: preg) (a: ireg) (rofs: ireg) (ofs: offset) (cp: compartment) (h priv: bool) :=
+  match Val.sub_offset_ptr (rs rofs) (eval_offset ofs) with
+  | Some ofsv => match Mem.loadv UNINIT chunk m (rs a) ofsv
+                                (if priv then None else Some cp) with
+                | inr PtrErr => Stuck
+                | inr CapErr => Crashed
+                | inl v => nextinstr (rs#d <- v) m
+                end
+  | _ => Stuck
+  end.
+
+Definition exec_load_ddc (chunk: cap_memory_chunk) (rs: regset) (m: mem)
+           (d: preg) (a: ireg) (ofs: offset) (cp: compartment) (priv: bool) :=
+  (* calculate offset from a and ofs *)
+  match Val.offset_ptr (rs a) (eval_offset ofs) with
+  | Some ofsv => match Mem.loadv DEFAULT chunk m (rs DDC) ofsv
+                                (if priv then None else Some cp) with
+                | inr PtrErr => Stuck
+                | inr CapErr => Crashed
+                | inl v => nextinstr (rs#d <- v) m
+                end
   | None => Stuck
-  | Some m' => Next (nextinstr rs) m'
+  end.
+
+Definition exec_store_capability (chunk: cap_memory_chunk) (rs: regset) (m: mem)
+           (s: preg) (a: ireg) (ofs: offset) (cp: compartment) (h: bool) :=
+  match Val.offset_ptr (rs a) (eval_offset ofs) with
+  | Some c => match Mem.storev DIR chunk m c (zero_offset h) (rs s) cp with
+             | inr PtrErr => Stuck
+             | inr CapErr => Crashed
+             | inl (_,m') => nextinstr rs m'
+             end
+  | None => Stuck
+  end.
+
+Definition exec_store_Ucapability (chunk: cap_memory_chunk) (rs: regset) (m: mem)
+           (s: preg) (a: ireg) (rofs: ireg) (ofs: offset) (cp: compartment) (h: bool) :=
+  match Val.sub_offset_ptr (rs rofs) (eval_offset ofs) with
+  | Some ofsv => match Mem.storev UNINIT chunk m (rs a) ofsv (rs s) cp with
+                | inr PtrErr => Stuck
+                | inr CapErr => Crashed
+                | inl (c',m') => nextinstr (rs#s <- (OCVcap c')) m'
+                end
+  | None => Stuck
+  end.
+
+Definition exec_store_ddc (chunk: cap_memory_chunk) (rs: regset) (m: mem)
+           (s: preg) (a: ireg) (ofs: offset) (cp: compartment) :=
+  (* calculate offset from a and ofs *)
+  match Val.offset_ptr (rs a) (eval_offset ofs) with
+  | Some ofsv => match Mem.storev DEFAULT chunk m (rs DDC) ofsv (rs s) cp with
+                | inr PtrErr => Stuck
+                | inr CapErr => Crashed
+                | inl (_,m') => nextinstr rs m'
+                end
+  | None => Stuck
   end.
 
 (** Evaluating a branch *)
@@ -750,9 +925,88 @@ Definition exec_store (chunk: memory_chunk) (rs: regset) (m: mem)
 Definition eval_branch (f: function) (l: label) (rs: regset) (m: mem) (res: option bool) : outcome :=
   match res with
     | Some true  => goto_label f l rs m
-    | Some false => Next (nextinstr rs) m
+    | Some false => nextinstr rs m
     | None => Stuck
   end.
+
+Definition eval_ptr_branch (f: function) (l1 l2: label) (rs: regset) (m: mem) (ptr: ocval) : outcome :=
+  match ptr with
+  | OCVptr (stack_ptr _) => goto_label f l1 rs m
+  | OCVptr (heap_ptr _) => goto_label f l2 rs m
+  | _ => nextinstr rs m
+  end.
+
+Definition exec_jal (rs: regset) (m: mem) (t: ocval) : outcome :=
+  match Val.offset_ptr rs#PCC Ptrofs.one with 
+  | Some ret => Next (rs#PCC <- (Val.update_pc_perm t) #RAC <- ret) m
+  | _ => Crashed
+  end.
+
+Definition exec_jal_seal (rs: regset) (m: mem) (t s: ocval) : outcome :=
+  match offset_ptr rs#PCC Ptrofs.one with
+  | Some ret => match Val.seal_capability ret s with
+               | Some res => Next (rs#PCC <- (update_pc_perm t) #RAC <- res) m
+               | _ => Crashed
+               end
+  | _ => Crashed
+  end.
+
+(** Clearing registers *)
+Arguments cons & _ _ _.
+
+
+(* AINA: how to make coercions work within list constructor? *)
+Fixpoint list_ip_coercion (l: list ireg) : list preg :=
+  match l with
+  | a :: l' => a :: list_ip_coercion l'
+  | nil => nil
+  end.
+Fixpoint list_fp_coercion (l: list freg) : list preg :=
+  match l with
+  | a :: l' => a :: list_fp_coercion l'
+  | nil => nil
+  end.
+
+(* AINA: the following is a bit hardcoded.. see if there is a better way of doing it *)
+Definition int_regs : list ireg :=
+  X1::X2::X3::X4::X5::X6::X7::X8::X9::X10::X11::X12::X13::X14::X15::X16::X17::X18::X19::
+  X20::X21::X22::X23::X24::X25::X26::X27::X28::X29::X30::X31::nil.
+Definition float_regs : list freg :=
+  F0::F1::F2::F3::F4::F5::F6::F7::F8::F9::F10::F11::F12::F13::F14::F15::F16::F17::F18::F19::
+  F20::F21::F22::F23::F24::F25::F26::F27::F28::F29::F30::F31::nil.
+
+Fixpoint filter_index {A: Type} (l: list A) (idx: list nat) : list A :=
+  match idx with
+  | nil => nil
+  | i :: idx' => match nth_error l i with
+               | Some a => a :: filter_index l idx'
+               | None => filter_index l idx'
+               end
+  end.
+
+Definition clear_registers (rs: regset) (vec: int) (is_int: bool) : regset :=
+  if is_int
+  then (* we shift vec in case of iregs to skip X0 *)
+    let idx := List.map Z.to_nat (Zbits.Z_one_bits Int.wordsize (Int.unsigned vec / 2) 0) in
+    let regs := list_ip_coercion (filter_index int_regs idx) in
+    set_regs_default regs (OCVint Int.zero) rs
+  else
+    let idx := List.map Z.to_nat (Zbits.Z_one_bits Int.wordsize (Int.unsigned vec) 0) in
+    let regs := list_fp_coercion (filter_index float_regs idx) in
+    set_regs_default regs (OCVint Int.zero) rs.
+
+(** Auxiliary definition that interprets partial operations into outcomes *)
+
+Definition exec_capability_outcome {A: Type} (v: option A) (rso: A -> outcome) : outcome :=
+  match v with
+  | Some res => rso res
+  | None => Crashed
+  end.
+
+Definition ptrofs_heap_res (ofs: ptrofs) : ocval :=
+  OCVptr (heap_ptr ofs).
+Definition ptrofs_stack_res (ofs: ptrofs) : ocval :=
+  OCVptr (stack_ptr ofs).
 
 (** Execution of a single instruction [i] in initial state [rs] and
     [m].  Return updated state.  For instructions that correspond to
@@ -769,152 +1023,158 @@ Definition eval_branch (f: function) (l: label) (rs: regset) (m: mem) (res: opti
 Definition exec_instr (f: function) (i: instruction) (rs: regset) (m: mem) (cp: compartment) : outcome :=
   match i with
   | Pmv d s =>
-      Next (nextinstr (rs#d <- (rs#s))) m
+      nextinstr (rs#d <- (rs#s)) m
 
 (** 32-bit integer register-immediate instructions *)
   | Paddiw d s i =>
-      Next (nextinstr (rs#d <- (Val.add rs##s (Vint i)))) m
+      nextinstr (rs#d <- (Val.add rs##s (OCVint i))) m
   | Psltiw d s i =>
-      Next (nextinstr (rs#d <- (Val.cmp Clt rs##s (Vint i)))) m
-  | Psltiuw d s i =>
-      Next (nextinstr (rs#d <- (Val.cmpu (Mem.valid_pointer m) Clt rs##s (Vint i)))) m
+      nextinstr (rs#d <- (Val.cmp Clt rs##s (OCVint i))) m
+  | Psltiuw d s i => (* ALG: ?? -- uses memory model *)
+      nextinstr (rs#d <- (Val.cmpu (Mem.valid_pointer m) Clt rs##s (OCVint i))) m
   | Pandiw d s i =>
-      Next (nextinstr (rs#d <- (Val.and rs##s (Vint i)))) m
+      nextinstr (rs#d <- (Val.and rs##s (OCVint i))) m
   | Poriw d s i =>
-      Next (nextinstr (rs#d <- (Val.or rs##s (Vint i)))) m
+      nextinstr (rs#d <- (Val.or rs##s (OCVint i))) m
   | Pxoriw d s i =>
-      Next (nextinstr (rs#d <- (Val.xor rs##s (Vint i)))) m
+      nextinstr (rs#d <- (Val.xor rs##s (OCVint i))) m
   | Pslliw d s i =>
-      Next (nextinstr (rs#d <- (Val.shl rs##s (Vint i)))) m
+      nextinstr (rs#d <- (Val.shl rs##s (OCVint i))) m
   | Psrliw d s i =>
-      Next (nextinstr (rs#d <- (Val.shru rs##s (Vint i)))) m
+      nextinstr (rs#d <- (Val.shru rs##s (OCVint i))) m
   | Psraiw d s i =>
-      Next (nextinstr (rs#d <- (Val.shr rs##s (Vint i)))) m
+      nextinstr (rs#d <- (Val.shr rs##s (OCVint i))) m
   | Pluiw d i =>
-      Next (nextinstr (rs#d <- (Vint (Int.shl i (Int.repr 12))))) m
+      nextinstr (rs#d <- (OCVint (Int.shl i (Int.repr 12)))) m
 
 (** 32-bit integer register-register instructions *)
   | Paddw d s1 s2 =>
-      Next (nextinstr (rs#d <- (Val.add rs##s1 rs##s2))) m
+       (nextinstr (rs#d <- (Val.add rs##s1 rs##s2))) m
   | Psubw d s1 s2 =>
-      Next (nextinstr (rs#d <- (Val.sub rs##s1 rs##s2))) m
+       (nextinstr (rs#d <- (Val.sub rs##s1 rs##s2))) m
   | Pmulw d s1 s2 =>
-      Next (nextinstr (rs#d <- (Val.mul rs##s1 rs##s2))) m
+       (nextinstr (rs#d <- (Val.mul rs##s1 rs##s2))) m
   | Pmulhw d s1 s2 =>
-      Next (nextinstr (rs#d <- (Val.mulhs rs##s1 rs##s2))) m
+       (nextinstr (rs#d <- (Val.mulhs rs##s1 rs##s2))) m
   | Pmulhuw d s1 s2 =>
-      Next (nextinstr (rs#d <- (Val.mulhu rs##s1 rs##s2))) m
+       (nextinstr (rs#d <- (Val.mulhu rs##s1 rs##s2))) m
   | Pdivw d s1 s2 =>
-      Next (nextinstr (rs#d <- (Val.maketotal (Val.divs rs##s1 rs##s2)))) m
+       (nextinstr (rs#d <- (Val.maketotal (Val.divs rs##s1 rs##s2)))) m
   | Pdivuw d s1 s2 =>
-      Next (nextinstr (rs#d <- (Val.maketotal (Val.divu rs##s1 rs##s2)))) m
+       (nextinstr (rs#d <- (Val.maketotal (Val.divu rs##s1 rs##s2)))) m
   | Premw d s1 s2 =>
-      Next (nextinstr (rs#d <- (Val.maketotal (Val.mods rs##s1 rs##s2)))) m
+       (nextinstr (rs#d <- (Val.maketotal (Val.mods rs##s1 rs##s2)))) m
   | Premuw d s1 s2 =>
-      Next (nextinstr (rs#d <- (Val.maketotal (Val.modu rs##s1 rs##s2)))) m
+       (nextinstr (rs#d <- (Val.maketotal (Val.modu rs##s1 rs##s2)))) m
   | Psltw d s1 s2 =>
-      Next (nextinstr (rs#d <- (Val.cmp Clt rs##s1 rs##s2))) m
+       (nextinstr (rs#d <- (Val.cmp Clt rs##s1 rs##s2))) m
   | Psltuw d s1 s2 =>
-      Next (nextinstr (rs#d <- (Val.cmpu (Mem.valid_pointer m) Clt rs##s1 rs##s2))) m
+       (nextinstr (rs#d <- (Val.cmpu (Mem.valid_pointer m) Clt rs##s1 rs##s2))) m
   | Pseqw d s1 s2 =>
-      Next (nextinstr (rs#d <- (Val.cmpu (Mem.valid_pointer m) Ceq rs##s1 rs##s2))) m
+       (nextinstr (rs#d <- (Val.cmpu (Mem.valid_pointer m) Ceq rs##s1 rs##s2))) m
   | Psnew d s1 s2 =>
-      Next (nextinstr (rs#d <- (Val.cmpu (Mem.valid_pointer m) Cne rs##s1 rs##s2))) m
+       (nextinstr (rs#d <- (Val.cmpu (Mem.valid_pointer m) Cne rs##s1 rs##s2))) m
   | Pandw d s1 s2 =>
-      Next (nextinstr (rs#d <- (Val.and rs##s1 rs##s2))) m
+       (nextinstr (rs#d <- (Val.and rs##s1 rs##s2))) m
   | Porw d s1 s2 =>
-      Next (nextinstr (rs#d <- (Val.or rs##s1 rs##s2))) m
+       (nextinstr (rs#d <- (Val.or rs##s1 rs##s2))) m
   | Pxorw d s1 s2 =>
-      Next (nextinstr (rs#d <- (Val.xor rs##s1 rs##s2))) m
+       (nextinstr (rs#d <- (Val.xor rs##s1 rs##s2))) m
   | Psllw d s1 s2 =>
-      Next (nextinstr (rs#d <- (Val.shl rs##s1 rs##s2))) m
+       (nextinstr (rs#d <- (Val.shl rs##s1 rs##s2))) m
   | Psrlw d s1 s2 =>
-      Next (nextinstr (rs#d <- (Val.shru rs##s1 rs##s2))) m
+       (nextinstr (rs#d <- (Val.shru rs##s1 rs##s2))) m
   | Psraw d s1 s2 =>
-      Next (nextinstr (rs#d <- (Val.shr rs##s1 rs##s2))) m
+       (nextinstr (rs#d <- (Val.shr rs##s1 rs##s2))) m
 
 (** 64-bit integer register-immediate instructions *)
   | Paddil d s i =>
-      Next (nextinstr (rs#d <- (Val.addl rs###s (Vlong i)))) m
+       (nextinstr (rs#d <- (Val.addl rs###s (OCVlong i)))) m
   | Psltil d s i =>
-      Next (nextinstr (rs#d <- (Val.maketotal (Val.cmpl Clt rs###s (Vlong i))))) m
+       (nextinstr (rs#d <- (Val.maketotal (Val.cmpl Clt rs###s (OCVlong i))))) m
   | Psltiul d s i =>
-      Next (nextinstr (rs#d <- (Val.maketotal (Val.cmplu (Mem.valid_pointer m) Clt rs###s (Vlong i))))) m
+       (nextinstr (rs#d <- (Val.maketotal (Val.cmplu (Mem.valid_pointer m) Clt rs###s (OCVlong i))))) m
   | Pandil d s i =>
-      Next (nextinstr (rs#d <- (Val.andl rs###s (Vlong i)))) m
+       (nextinstr (rs#d <- (Val.andl rs###s (OCVlong i)))) m
   | Poril d s i =>
-      Next (nextinstr (rs#d <- (Val.orl rs###s (Vlong i)))) m
+       (nextinstr (rs#d <- (Val.orl rs###s (OCVlong i)))) m
   | Pxoril d s i =>
-      Next (nextinstr (rs#d <- (Val.xorl rs###s (Vlong i)))) m
+       (nextinstr (rs#d <- (Val.xorl rs###s (OCVlong i)))) m
   | Psllil d s i =>
-      Next (nextinstr (rs#d <- (Val.shll rs###s (Vint i)))) m
+       (nextinstr (rs#d <- (Val.shll rs###s (OCVint i)))) m
   | Psrlil d s i =>
-      Next (nextinstr (rs#d <- (Val.shrlu rs###s (Vint i)))) m
+       (nextinstr (rs#d <- (Val.shrlu rs###s (OCVint i)))) m
   | Psrail d s i =>
-      Next (nextinstr (rs#d <- (Val.shrl rs###s (Vint i)))) m
+       (nextinstr (rs#d <- (Val.shrl rs###s (OCVint i)))) m
   | Pluil d i =>
-      Next (nextinstr (rs#d <- (Vlong (Int64.sign_ext 32 (Int64.shl i (Int64.repr 12)))))) m
+       (nextinstr (rs#d <- (OCVlong (Int64.sign_ext 32 (Int64.shl i (Int64.repr 12)))))) m
 
 (** 64-bit integer register-register instructions *)
   | Paddl d s1 s2 =>
-      Next (nextinstr (rs#d <- (Val.addl rs###s1 rs###s2))) m
+       (nextinstr (rs#d <- (Val.addl rs###s1 rs###s2))) m
   | Psubl d s1 s2 =>
-      Next (nextinstr (rs#d <- (Val.subl rs###s1 rs###s2))) m
+       (nextinstr (rs#d <- (Val.subl rs###s1 rs###s2))) m
   | Pmull d s1 s2 =>
-      Next (nextinstr (rs#d <- (Val.mull rs###s1 rs###s2))) m
+       (nextinstr (rs#d <- (Val.mull rs###s1 rs###s2))) m
   | Pmulhl d s1 s2 =>
-      Next (nextinstr (rs#d <- (Val.mullhs rs###s1 rs###s2))) m
+       (nextinstr (rs#d <- (Val.mullhs rs###s1 rs###s2))) m
   | Pmulhul d s1 s2 =>
-      Next (nextinstr (rs#d <- (Val.mullhu rs###s1 rs###s2))) m
+       (nextinstr (rs#d <- (Val.mullhu rs###s1 rs###s2))) m
   | Pdivl d s1 s2 =>
-      Next (nextinstr (rs#d <- (Val.maketotal (Val.divls rs###s1 rs###s2)))) m
+       (nextinstr (rs#d <- (Val.maketotal (Val.divls rs###s1 rs###s2)))) m
   | Pdivul d s1 s2 =>
-      Next (nextinstr (rs#d <- (Val.maketotal (Val.divlu rs###s1 rs###s2)))) m
+       (nextinstr (rs#d <- (Val.maketotal (Val.divlu rs###s1 rs###s2)))) m
   | Preml d s1 s2 =>
-      Next (nextinstr (rs#d <- (Val.maketotal (Val.modls rs###s1 rs###s2)))) m
+       (nextinstr (rs#d <- (Val.maketotal (Val.modls rs###s1 rs###s2)))) m
   | Premul d s1 s2 =>
-      Next (nextinstr (rs#d <- (Val.maketotal (Val.modlu rs###s1 rs###s2)))) m
+       (nextinstr (rs#d <- (Val.maketotal (Val.modlu rs###s1 rs###s2)))) m
   | Psltl d s1 s2 =>
-      Next (nextinstr (rs#d <- (Val.maketotal (Val.cmpl Clt rs###s1 rs###s2)))) m
+       (nextinstr (rs#d <- (Val.maketotal (Val.cmpl Clt rs###s1 rs###s2)))) m
   | Psltul d s1 s2 =>
-      Next (nextinstr (rs#d <- (Val.maketotal (Val.cmplu (Mem.valid_pointer m) Clt rs###s1 rs###s2)))) m
+       (nextinstr (rs#d <- (Val.maketotal (Val.cmplu (Mem.valid_pointer m) Clt rs###s1 rs###s2)))) m
   | Pseql d s1 s2 =>
-      Next (nextinstr (rs#d <- (Val.maketotal (Val.cmplu (Mem.valid_pointer m) Ceq rs###s1 rs###s2)))) m
+       (nextinstr (rs#d <- (Val.maketotal (Val.cmplu (Mem.valid_pointer m) Ceq rs###s1 rs###s2)))) m
   | Psnel d s1 s2 =>
-      Next (nextinstr (rs#d <- (Val.maketotal (Val.cmplu (Mem.valid_pointer m) Cne rs###s1 rs###s2)))) m
+       (nextinstr (rs#d <- (Val.maketotal (Val.cmplu (Mem.valid_pointer m) Cne rs###s1 rs###s2)))) m
   | Pandl d s1 s2 =>
-      Next (nextinstr (rs#d <- (Val.andl rs###s1 rs###s2))) m
+       (nextinstr (rs#d <- (Val.andl rs###s1 rs###s2))) m
   | Porl d s1 s2 =>
-      Next (nextinstr (rs#d <- (Val.orl rs###s1 rs###s2))) m
+       (nextinstr (rs#d <- (Val.orl rs###s1 rs###s2))) m
   | Pxorl d s1 s2 =>
-      Next (nextinstr (rs#d <- (Val.xorl rs###s1 rs###s2))) m
+       (nextinstr (rs#d <- (Val.xorl rs###s1 rs###s2))) m
   | Pslll d s1 s2 =>
-      Next (nextinstr (rs#d <- (Val.shll rs###s1 rs###s2))) m
+       (nextinstr (rs#d <- (Val.shll rs###s1 rs###s2))) m
   | Psrll d s1 s2 =>
-      Next (nextinstr (rs#d <- (Val.shrlu rs###s1 rs###s2))) m
+       (nextinstr (rs#d <- (Val.shrlu rs###s1 rs###s2))) m
   | Psral d s1 s2 =>
-      Next (nextinstr (rs#d <- (Val.shrl rs###s1 rs###s2))) m
+       (nextinstr (rs#d <- (Val.shrl rs###s1 rs###s2))) m
 
   | Pcvtl2w d s =>
-      Next (nextinstr (rs#d <- (Val.loword rs##s))) m
+       (nextinstr (rs#d <- (Val.loword rs##s))) m
   | Pcvtw2l r =>
-      Next (nextinstr (rs#r <- (Val.longofint rs#r))) m
+       (nextinstr (rs#r <- (Val.longofint rs#r))) m
 
 (** Unconditional jumps.  Links are always to X1/RA. *)
   | Pj_l l =>
       goto_label f l rs m
-  | Pj_s s sg =>
-      Next (rs#PC <- (Genv.symbol_address ge s Ptrofs.zero)) m
-  | Pj_r r sg _ =>
-      Next (rs#PC <- (rs#r)) m
-  | Pjal_s s sg _ =>
-    Next (rs#PC <- (Genv.symbol_address ge s Ptrofs.zero)
-            #RA <- (Val.offset_ptr rs#PC Ptrofs.one)
-         ) m
+  (* | Pj_s s sg => *)
+  (*    Next (rs#PCC <- (update_pc_perm (Genv.symbol_address ge s Ptrofs.zero))) m *)
+  | Pj_r r =>
+      Next (rs#PCC <- (update_pc_perm (rs#r))) m
+  (* | Pjal_s s sg _ => *)
+  (*     exec_jal rs m (Genv.symbol_address ge s Ptrofs.zero) *)
   | Pjal_r r sg _ =>
-      Next (rs#PC <- (rs#r)
-              #RA <- (Val.offset_ptr rs#PC Ptrofs.one)
-           ) m
+      exec_jal rs m (rs#r)
+  | PCjal_r r s _ _ =>
+      exec_jal_seal rs m (rs#r) (rs#s)
+  (* | PCjal_s f s _ _ => *)
+  (*     exec_jal_seal rs m (Genv.symbol_address ge f Ptrofs.zero) (rs#s) *)
+
+(** Sealed capability invocation *)
+  | PCinvoke r s _ =>
+      exec_capability_outcome (Val.unseal_capability_pair (rs##r) (rs##s))
+                              (fun c => Next (rs#PCC <- (fst c) #EC <- (snd c)) m)
+      
 (** Conditional branches, 32-bit comparisons *)
   | Pbeqw s1 s2 l =>
       eval_branch f l rs m (Val.cmpu_bool (Mem.valid_pointer m) Ceq rs##s1 rs##s2)
@@ -945,182 +1205,403 @@ Definition exec_instr (f: function) (i: instruction) (rs: regset) (m: mem) (cp: 
 
 (** Loads and stores *)
   | Plb d a ofs priv =>
-      exec_load Mint8signed rs m d a ofs cp priv
+      exec_load_ddc CMint8signed rs m d a ofs cp priv
   | Plbu d a ofs priv =>
-      exec_load Mint8unsigned rs m d a ofs cp priv
+      exec_load_ddc CMint8unsigned rs m d a ofs cp priv
   | Plh d a ofs priv =>
-      exec_load Mint16signed rs m d a ofs cp priv
+      exec_load_ddc CMint16signed rs m d a ofs cp priv
   | Plhu d a ofs priv =>
-      exec_load Mint16unsigned rs m d a ofs cp priv
+      exec_load_ddc CMint16unsigned rs m d a ofs cp priv
   | Plw d a ofs priv =>
-      exec_load Mint32 rs m d a ofs cp priv
+      exec_load_ddc CMint32 rs m d a ofs cp priv
   | Plw_a d a ofs priv =>
-      exec_load Many32 rs m d a ofs cp priv
+      exec_load_ddc CMany32 rs m d a ofs cp priv
   | Pld d a ofs priv =>
-      exec_load Mint64 rs m d a ofs cp priv
+      exec_load_ddc CMint64 rs m d a ofs cp priv
   | Pld_a d a ofs priv =>
-      exec_load Many64 rs m d a ofs cp priv
+      exec_load_ddc CMany64 rs m d a ofs cp priv
+  | Plcw d a ofs priv =>
+      exec_load_ddc CMcap64 rs m d a ofs cp priv
+  | Plcd d a ofs priv =>
+      exec_load_ddc CMcap128 rs m d a ofs cp priv
+  | Plcd_a d a ofs priv =>
+      exec_load_ddc CMany128 rs m d a ofs cp priv
+  
   | Psb s a ofs =>
-      exec_store Mint8unsigned rs m s a ofs cp
+      exec_store_ddc CMint8unsigned rs m s a ofs cp
   | Psh s a ofs =>
-      exec_store Mint16unsigned rs m s a ofs cp
+      exec_store_ddc CMint16unsigned rs m s a ofs cp
   | Psw s a ofs =>
-      exec_store Mint32 rs m s a ofs cp
+      exec_store_ddc CMint32 rs m s a ofs cp
   | Psw_a s a ofs =>
-      exec_store Many32 rs m s a ofs cp
+      exec_store_ddc CMany32 rs m s a ofs cp
   | Psd s a ofs =>
-      exec_store Mint64 rs m s a ofs cp
+      exec_store_ddc CMint64 rs m s a ofs cp
   | Psd_a s a ofs =>
-      exec_store Many64 rs m s a ofs cp
+      exec_store_ddc CMany64 rs m s a ofs cp
+  | Pscw s a ofs =>
+      exec_store_ddc CMcap64 rs m s a ofs cp
+  | Pscd s a ofs =>
+      exec_store_ddc CMcap128 rs m s a ofs cp
+  | Pscd_a s a ofs =>
+      exec_store_ddc CMany128 rs m s a ofs cp
 
+(** Capability loads and stores *)
+  | PClb d a ofs h priv =>
+      exec_load_capability CMint8signed rs m d a ofs cp h priv
+  | PClbu d a ofs h priv =>
+      exec_load_capability CMint8unsigned rs m d a ofs cp h priv
+  | PClh d a ofs h priv =>
+      exec_load_capability CMint16signed rs m d a ofs cp h priv
+  | PClhu d a ofs h priv =>
+      exec_load_capability CMint16unsigned rs m d a ofs cp h priv
+  | PClw d a ofs h priv =>
+      exec_load_capability CMint32 rs m d a ofs cp h priv
+  | PClw_a d a ofs h priv =>
+      exec_load_capability CMany32 rs m d a ofs cp h priv
+  | PCld d a ofs h priv =>
+      exec_load_capability CMint64 rs m d a ofs cp h priv
+  | PCld_a d a ofs h priv =>
+      exec_load_capability CMany64 rs m d a ofs cp h priv
+  | PClwc d a ofs h priv =>
+      exec_load_capability CMcap64 rs m d a ofs cp h priv
+  | PClcd d a ofs h priv =>
+      exec_load_capability CMcap128 rs m d a ofs cp h priv
+  | PClcd_a d a ofs h priv =>
+      exec_load_capability CMany128 rs m d a ofs cp h priv
+            
+  | PCsb s a ofs h =>
+      exec_store_capability CMint8unsigned rs m s a ofs cp h
+  | PCsh s a ofs h =>
+      exec_store_capability CMint16unsigned rs m s a ofs cp h
+  | PCsw s a ofs h =>
+      exec_store_capability CMint32 rs m s a ofs cp h
+  | PCsw_a s a ofs h =>
+      exec_store_capability CMany32 rs m s a ofs cp h
+  | PCsd s a ofs h =>
+      exec_store_capability CMint64 rs m s a ofs cp h
+  | PCsd_a s a ofs h =>
+      exec_store_capability CMany64 rs m s a ofs cp h
+  | PCscw s a ofs h =>
+      exec_store_capability CMcap64 rs m s a ofs cp h
+  | PCscd s a ofs h =>
+      exec_store_capability CMcap128 rs m s a ofs cp h
+  | PCscd_a s a ofs h =>
+      exec_store_capability CMany128 rs m s a ofs cp h
+
+  | PCfls d a ofs h priv =>
+      exec_load_capability CMfloat32 rs m d a ofs cp h priv
+  | PCfss s a ofs h =>
+      exec_store_capability CMfloat32 rs m s a ofs cp h
+  | PCfld d a ofs h priv =>
+      exec_load_capability CMfloat64 rs m d a ofs cp h priv
+  | PCfld_a d a ofs h priv =>
+      exec_load_capability CMany64 rs m d a ofs cp h priv
+  | PCfsd s a ofs h =>
+      exec_store_capability CMfloat64 rs m s a ofs cp h
+  | PCfsd_a s a ofs h =>
+      exec_store_capability CMany64 rs m s a ofs cp h
+                            
+  (** Uninitialized Capability loads and stores *)
+  | PCUlb d a rofs ofs h priv =>
+      exec_load_Ucapability CMint8signed rs m d a rofs ofs cp h priv
+  | PCUlbu d a rofs ofs h priv =>
+      exec_load_Ucapability CMint8unsigned rs m d a rofs ofs cp h priv
+  | PCUlh d a rofs ofs h priv =>
+      exec_load_Ucapability CMint16signed rs m d a rofs ofs cp h priv
+  | PCUlhu d a rofs ofs h priv =>
+      exec_load_Ucapability CMint16unsigned rs m d a rofs ofs cp h priv
+  | PCUlw d a rofs ofs h priv =>
+      exec_load_Ucapability CMint32 rs m d a rofs ofs cp h priv
+  | PCUlw_a d a rofs ofs h priv =>
+      exec_load_Ucapability CMany32 rs m d a rofs ofs cp h priv
+  | PCUld d a rofs ofs h priv =>
+      exec_load_Ucapability CMint64 rs m d a rofs ofs cp h priv
+  | PCUld_a d a rofs ofs h priv =>
+      exec_load_Ucapability CMany64 rs m d a rofs ofs cp h priv
+  | PCUlwc d a rofs ofs h priv =>
+      exec_load_Ucapability CMcap64 rs m d a rofs ofs cp h priv
+  | PCUlcd d a rofs ofs h priv =>
+      exec_load_Ucapability CMcap128 rs m d a rofs ofs cp h priv
+  | PCUlcd_a d a rofs ofs h priv =>
+      exec_load_Ucapability CMany128 rs m d a rofs ofs cp h priv
+            
+  | PCUsb s a rofs ofs h =>
+      exec_store_Ucapability CMint8unsigned rs m s a rofs ofs cp h
+  | PCUsh s a rofs ofs h =>
+      exec_store_Ucapability CMint16unsigned rs m s a rofs ofs cp h
+  | PCUsw s a rofs ofs h =>
+      exec_store_Ucapability CMint32 rs m s a rofs ofs cp h
+  | PCUsw_a s a rofs ofs h =>
+      exec_store_Ucapability CMany32 rs m s a rofs ofs cp h
+  | PCUsd s a rofs ofs h =>
+      exec_store_Ucapability CMint64 rs m s a rofs ofs cp h
+  | PCUsd_a s a rofs ofs h =>
+      exec_store_Ucapability CMany64 rs m s a rofs ofs cp h
+  | PCUscw s a rofs ofs h =>
+      exec_store_Ucapability CMcap64 rs m s a rofs ofs cp h
+  | PCUscd s a rofs ofs h =>
+      exec_store_Ucapability CMcap128 rs m s a rofs ofs cp h
+  | PCUscd_a s a rofs ofs h =>
+      exec_store_Ucapability CMany128 rs m s a rofs ofs cp h
+
+  | PCUfls d a rofs ofs h priv =>
+      exec_load_Ucapability CMfloat32 rs m d a rofs ofs cp h priv
+  | PCUfss s a rofs ofs h =>
+      exec_store_Ucapability CMfloat32 rs m s a rofs ofs cp h
+  | PCUfld d a rofs ofs h priv =>
+      exec_load_Ucapability CMfloat64 rs m d a rofs ofs cp h priv
+  | PCUfld_a d a rofs ofs h priv =>
+      exec_load_Ucapability CMany64 rs m d a rofs ofs cp h priv
+  | PCUfsd s a rofs ofs h =>
+      exec_store_Ucapability CMfloat64 rs m s a rofs ofs cp h
+  | PCUfsd_a s a rofs ofs h =>
+      exec_store_Ucapability CMany64 rs m s a rofs ofs cp h
+                             
+(** Capability inspection *)
+  | PCgp d s =>
+      Next (rs#d <- (Val.maketotal (do X <- get_cap rs#s >>= get_perm; Some (encode_perm X)))) m
+  | PCgt d s =>
+      Next (rs#d <- (Val.maketotal (do X <- get_cap rs#s >>= get_otype; Some (OCVint (Ptrofs.to_int X))))) m
+  | PCgb_h d s =>
+      Next (rs#d <- (Val.maketotal (do X <- get_cap rs#s; Some (ptrofs_heap_res (get_lo X))))) m
+  | PCge_h d s =>
+      Next (rs#d <- (Val.maketotal (do X <- get_cap rs#s; Some (ptrofs_heap_res (get_hi X))))) m
+  | PCgb_s d s =>
+      Next (rs#d <- (Val.maketotal (do X <- get_cap rs#s; Some (ptrofs_stack_res (get_lo X))))) m
+  | PCge_s d s =>
+      Next (rs#d <- (Val.maketotal (do X <- get_cap rs#s; Some (ptrofs_stack_res (get_hi X))))) m
+  | PCgg d s =>
+      Next (rs#d <- (OCVint (Int.repr (Z.b2z (is_cap_b rs#s))))) m
+  | PCgs d s =>
+      Next (rs#d <- (OCVint (Int.repr (Z.b2z (is_sealed_cap rs#s))))) m
+  | PCga_h d s =>
+      Next (rs#d <- (Val.maketotal (do X <- get_cap rs#s; Some (ptrofs_heap_res (get_addr X))))) m
+  | PCga_s d s =>
+      Next (rs#d <- (Val.maketotal (do X <- get_cap rs#s; Some (ptrofs_stack_res (get_addr X))))) m
+  | PCgl_h d s =>
+      Next (rs#d <- (Val.maketotal (do X <- get_cap rs#s; Some (ptrofs_heap_res (get_region_size_ptrofs X))))) m
+  | PCgl_s d s =>
+      Next (rs#d <- (Val.maketotal (do X <- get_cap rs#s; Some (ptrofs_stack_res (get_region_size_ptrofs X))))) m
+
+(** Capability modification *)
+  | PCseal d r1 r2 =>
+      exec_capability_outcome (Val.seal_capability rs#r1 rs#r2) (fun b => Next (rs#d <- b) m)
+  | PCunseal d r1 r2 =>
+      exec_capability_outcome (Val.unseal_capability rs#r1 rs#r2) (fun b => Next (rs#d <- b) m)
+  | PCpermand d r1 r2 =>
+      exec_capability_outcome (Val.restrict_perm decode_perm_int rs#r1 rs#r2) (fun b => Next (rs#d <- b) m)
+  | PCsaddr_w d r1 r2 =>
+      exec_capability_outcome (Val.set_address rs#r1 rs#r2) (fun b => Next (rs#d <- b) m)
+  | PCsaddr_l d r1 r2 =>
+      exec_capability_outcome (Val.set_addressl rs#r1 rs#r2) (fun b => Next (rs#d <- b) m)
+  | PCiaddr_w d r1 r2 =>
+      exec_capability_outcome (Val.incr_address rs##r1 rs##r2) (fun b => Next (rs#d <- b) m)
+  | PCiaddr_l d r1 r2 =>
+      exec_capability_outcome (Val.incr_addressl rs##r1 rs##r2) (fun b => Next (rs#d <- b) m)
+  | PCiaddr_il d r1 imm =>
+      exec_capability_outcome (Val.incr_addressl rs##r1 (OCVlong imm)) (fun b => Next (rs#d <- b) m)
+  | PCiaddr_iw d r1 imm =>
+      exec_capability_outcome (Val.incr_address rs##r1 (OCVint imm)) (fun b => Next (rs#d <- b) m)
+  | PCsbase d r1 r2 =>
+      exec_capability_outcome (Val.sub_bounds rs#r1 rs#r2) (fun b => Next (rs#d <- b) m)
+  | PCsbase_il d r1 imm =>
+      exec_capability_outcome (Val.sub_bounds rs#r1 (OCVlong imm)) (fun b => Next (rs#d <- b) m)
+  | PCsbase_iw d r1 imm =>
+      exec_capability_outcome (Val.sub_bounds rs#r1 (OCVint imm)) (fun b => Next (rs#d <- b) m)
+  (* | PCcleart _ _ *) (* removed for now => needs some kind of
+  enconding from capabilities to integers, however issues with space:
+  the encoding has to go from a capability to two integers/two
+  longs *)
+  | PCCseal d r1 r2 =>
+      exec_capability_outcome (Val.conditional_seal_capability rs#r1 rs#r2) (fun b => Next (rs#d <- b) m)
+  | PCseal_e d r =>
+      exec_capability_outcome (Val.restrict_perm decode_perm_int rs#r (OCVint (encode_perm_int E)))
+                              (fun b => Next (rs#d <- b) m)
+  | PCpromote d r1 =>
+      exec_capability_outcome (Val.promote rs#r1) (fun b => Next (rs#d <- b) m)
+                              
+(** Capability arithmetic *)
+  | PCtoPtr_h d r1 r2 =>
+      exec_capability_outcome (Val.c_to_ptr_heap rs#r1 rs#r2) (fun b => Next (rs#d <- b) m)
+  | PCsub_h d r1 r2 =>
+      Next (rs#d <- (Val.capability_sub_heap rs#r1 rs#r2)) m
+  | PCtoPtr_s d r1 r2 =>
+      exec_capability_outcome (Val.c_to_ptr_stack rs#r1 rs#r2) (fun b => Next (rs#d <- b) m)
+  | PCsub_s d r1 r2 =>
+      Next (rs#d <- (Val.capability_sub_stack rs#r1 rs#r2)) m
+  | PCUtoPtr_h d r1 r2 =>
+      exec_capability_outcome (Val.c_to_Uptr_heap rs#r1 rs#r2) (fun b => Next (rs#d <- b) m)
+  | PCUtoPtr_s d r1 r2 => 
+      exec_capability_outcome (Val.c_to_Uptr_heap rs#r1 rs#r2) (fun b => Next (rs#d <- b) m)
+                              
+(** Capability comparisons *)
+  | PCsubset d r1 r2 =>
+      Next (rs#d <- (Val.maketotal (do X1 <- get_cap rs#r1;
+                                   do X2 <- get_cap rs#r2;
+                    Some (OCVint (Int.repr (Z.b2z (Mem.derived_cap_dec X1 X2))))))) m
+  | PCeex d r1 r2 =>
+      Next (rs#d <- (Val.maketotal (do X1 <- get_cap rs#r1;
+                                   do X2 <- get_cap rs#r2;
+                    Some (OCVint (Int.repr (Z.b2z (occap_dec X1 X2))))))) m
+
+(** Fast clearing *)
+  | PCCclear imm => Next (clear_registers rs imm true) m
+  | PCCclearf imm => Next (clear_registers rs imm false) m
+
+              
 (** Floating point register move *)
   | Pfmv d s =>
-      Next (nextinstr (rs#d <- (rs#s))) m
+      (nextinstr (rs#d <- (rs#s))) m
 
 (** 32-bit (single-precision) floating point *)
   | Pfls d a ofs b =>
-      exec_load Mfloat32 rs m d a ofs cp b
+      exec_load_ddc CMfloat32 rs m d a ofs cp b
   | Pfss s a ofs =>
-      exec_store Mfloat32 rs m s a ofs cp
+      exec_store_ddc CMfloat32 rs m s a ofs cp
 
   | Pfnegs d s =>
-      Next (nextinstr (rs#d <- (Val.negfs rs#s))) m
+      (nextinstr (rs#d <- (Val.negfs rs#s))) m
   | Pfabss d s =>
-      Next (nextinstr (rs#d <- (Val.absfs rs#s))) m
+      (nextinstr (rs#d <- (Val.absfs rs#s))) m
 
   | Pfadds d s1 s2 =>
-      Next (nextinstr (rs#d <- (Val.addfs rs#s1 rs#s2))) m
+       (nextinstr (rs#d <- (Val.addfs rs#s1 rs#s2))) m
   | Pfsubs d s1 s2 =>
-      Next (nextinstr (rs#d <- (Val.subfs rs#s1 rs#s2))) m
+       (nextinstr (rs#d <- (Val.subfs rs#s1 rs#s2))) m
   | Pfmuls d s1 s2 =>
-      Next (nextinstr (rs#d <- (Val.mulfs rs#s1 rs#s2))) m
+       (nextinstr (rs#d <- (Val.mulfs rs#s1 rs#s2))) m
   | Pfdivs d s1 s2 =>
-      Next (nextinstr (rs#d <- (Val.divfs rs#s1 rs#s2))) m
+       (nextinstr (rs#d <- (Val.divfs rs#s1 rs#s2))) m
   | Pfeqs d s1 s2 =>
-      Next (nextinstr (rs#d <- (Val.cmpfs Ceq rs#s1 rs#s2))) m
+       (nextinstr (rs#d <- (Val.cmpfs Ceq rs#s1 rs#s2))) m
   | Pflts d s1 s2 =>
-      Next (nextinstr (rs#d <- (Val.cmpfs Clt rs#s1 rs#s2))) m
+       (nextinstr (rs#d <- (Val.cmpfs Clt rs#s1 rs#s2))) m
   | Pfles d s1 s2 =>
-      Next (nextinstr (rs#d <- (Val.cmpfs Cle rs#s1 rs#s2))) m
+       (nextinstr (rs#d <- (Val.cmpfs Cle rs#s1 rs#s2))) m
 
   | Pfcvtws d s =>
-      Next (nextinstr (rs#d <- (Val.maketotal (Val.intofsingle rs#s)))) m
+       (nextinstr (rs#d <- (Val.maketotal (Val.intofsingle rs#s)))) m
   | Pfcvtwus d s =>
-      Next (nextinstr (rs#d <- (Val.maketotal (Val.intuofsingle rs#s)))) m
+       (nextinstr (rs#d <- (Val.maketotal (Val.intuofsingle rs#s)))) m
   | Pfcvtsw d s =>
-      Next (nextinstr (rs#d <- (Val.maketotal (Val.singleofint rs##s)))) m
+       (nextinstr (rs#d <- (Val.maketotal (Val.singleofint rs##s)))) m
   | Pfcvtswu d s =>
-      Next (nextinstr (rs#d <- (Val.maketotal (Val.singleofintu rs##s)))) m
+       (nextinstr (rs#d <- (Val.maketotal (Val.singleofintu rs##s)))) m
 
   | Pfcvtls d s =>
-      Next (nextinstr (rs#d <- (Val.maketotal (Val.longofsingle rs#s)))) m
+       (nextinstr (rs#d <- (Val.maketotal (Val.longofsingle rs#s)))) m
   | Pfcvtlus d s =>
-      Next (nextinstr (rs#d <- (Val.maketotal (Val.longuofsingle rs#s)))) m
+       (nextinstr (rs#d <- (Val.maketotal (Val.longuofsingle rs#s)))) m
   | Pfcvtsl d s =>
-      Next (nextinstr (rs#d <- (Val.maketotal (Val.singleoflong rs###s)))) m
+       (nextinstr (rs#d <- (Val.maketotal (Val.singleoflong rs###s)))) m
   | Pfcvtslu d s =>
-      Next (nextinstr (rs#d <- (Val.maketotal (Val.singleoflongu rs###s)))) m
+       (nextinstr (rs#d <- (Val.maketotal (Val.singleoflongu rs###s)))) m
 
 (** 64-bit (double-precision) floating point *)
   | Pfld d a ofs b =>
-      exec_load Mfloat64 rs m d a ofs cp b
+      exec_load_ddc CMfloat64 rs m d a ofs cp b
   | Pfld_a d a ofs b =>
-      exec_load Many64 rs m d a ofs cp b
+      exec_load_ddc CMany64 rs m d a ofs cp b
   | Pfsd s a ofs =>
-      exec_store Mfloat64 rs m s a ofs cp
+      exec_store_ddc CMfloat64 rs m s a ofs cp
   | Pfsd_a s a ofs =>
-      exec_store Many64 rs m s a ofs cp
+      exec_store_ddc CMany64 rs m s a ofs cp
 
   | Pfnegd d s =>
-      Next (nextinstr (rs#d <- (Val.negf rs#s))) m
+       (nextinstr (rs#d <- (Val.negf rs#s))) m
   | Pfabsd d s =>
-      Next (nextinstr (rs#d <- (Val.absf rs#s))) m
+       (nextinstr (rs#d <- (Val.absf rs#s))) m
 
   | Pfaddd d s1 s2 =>
-      Next (nextinstr (rs#d <- (Val.addf rs#s1 rs#s2))) m
+       (nextinstr (rs#d <- (Val.addf rs#s1 rs#s2))) m
   | Pfsubd d s1 s2 =>
-      Next (nextinstr (rs#d <- (Val.subf rs#s1 rs#s2))) m
+       (nextinstr (rs#d <- (Val.subf rs#s1 rs#s2))) m
   | Pfmuld d s1 s2 =>
-      Next (nextinstr (rs#d <- (Val.mulf rs#s1 rs#s2))) m
+       (nextinstr (rs#d <- (Val.mulf rs#s1 rs#s2))) m
   | Pfdivd d s1 s2 =>
-      Next (nextinstr (rs#d <- (Val.divf rs#s1 rs#s2))) m
+       (nextinstr (rs#d <- (Val.divf rs#s1 rs#s2))) m
   | Pfeqd d s1 s2 =>
-      Next (nextinstr (rs#d <- (Val.cmpf Ceq rs#s1 rs#s2))) m
+       (nextinstr (rs#d <- (Val.cmpf Ceq rs#s1 rs#s2))) m
   | Pfltd d s1 s2 =>
-      Next (nextinstr (rs#d <- (Val.cmpf Clt rs#s1 rs#s2))) m
+       (nextinstr (rs#d <- (Val.cmpf Clt rs#s1 rs#s2))) m
   | Pfled d s1 s2 =>
-      Next (nextinstr (rs#d <- (Val.cmpf Cle rs#s1 rs#s2))) m
+       (nextinstr (rs#d <- (Val.cmpf Cle rs#s1 rs#s2))) m
 
   | Pfcvtwd d s =>
-      Next (nextinstr (rs#d <- (Val.maketotal (Val.intoffloat rs#s)))) m
+       (nextinstr (rs#d <- (Val.maketotal (Val.intoffloat rs#s)))) m
   | Pfcvtwud d s =>
-      Next (nextinstr (rs#d <- (Val.maketotal (Val.intuoffloat rs#s)))) m
+       (nextinstr (rs#d <- (Val.maketotal (Val.intuoffloat rs#s)))) m
   | Pfcvtdw d s =>
-      Next (nextinstr (rs#d <- (Val.maketotal (Val.floatofint rs##s)))) m
+       (nextinstr (rs#d <- (Val.maketotal (Val.floatofint rs##s)))) m
   | Pfcvtdwu d s =>
-      Next (nextinstr (rs#d <- (Val.maketotal (Val.floatofintu rs##s)))) m
+       (nextinstr (rs#d <- (Val.maketotal (Val.floatofintu rs##s)))) m
 
   | Pfcvtld d s =>
-      Next (nextinstr (rs#d <- (Val.maketotal (Val.longoffloat rs#s)))) m
+       (nextinstr (rs#d <- (Val.maketotal (Val.longoffloat rs#s)))) m
   | Pfcvtlud d s =>
-      Next (nextinstr (rs#d <- (Val.maketotal (Val.longuoffloat rs#s)))) m
+       (nextinstr (rs#d <- (Val.maketotal (Val.longuoffloat rs#s)))) m
   | Pfcvtdl d s =>
-      Next (nextinstr (rs#d <- (Val.maketotal (Val.floatoflong rs###s)))) m
+       (nextinstr (rs#d <- (Val.maketotal (Val.floatoflong rs###s)))) m
   | Pfcvtdlu d s =>
-      Next (nextinstr (rs#d <- (Val.maketotal (Val.floatoflongu rs###s)))) m
+       (nextinstr (rs#d <- (Val.maketotal (Val.floatoflongu rs###s)))) m
 
   | Pfcvtds d s =>
-      Next (nextinstr (rs#d <- (Val.floatofsingle rs#s))) m
+       (nextinstr (rs#d <- (Val.floatofsingle rs#s))) m
   | Pfcvtsd d s =>
-      Next (nextinstr (rs#d <- (Val.singleoffloat rs#s))) m
+       (nextinstr (rs#d <- (Val.singleoffloat rs#s))) m
 
 (** Pseudo-instructions *)
-  | Pallocframe sz pos =>
-      let (m1, stk) := Mem.alloc m (comp_of f) 0 sz in
-      let sp := (Vptr stk Ptrofs.zero) in
-      match Mem.storev Mptr m1 (Val.offset_ptr sp pos) rs#SP cp with
-      | None => Stuck
-      | Some m2 => Next (nextinstr (rs #X30 <- (rs SP) #SP <- sp #X31 <- Vundef)) m2
-      end
-  | Pfreeframe sz pos =>
-      match Mem.loadv Mptr m (Val.offset_ptr rs#SP pos) (Some cp) with
-      | None => Stuck
-      | Some v =>
-          match rs SP with
-          | Vptr stk ofs =>
-              match Mem.free m stk 0 sz cp with
-              | None => Stuck
-              | Some m' => Next (nextinstr (rs#SP <- v #X31 <- Vundef)) m'
-              end
-          | _ => Stuck
-          end
-      end
+  (* | Pallocframe sz pos => *)
+  (*     let (m1, stk) := Mem.alloc m (comp_of f) 0 sz in *)
+  (*     let sp := (Vptr stk Ptrofs.zero) in *)
+  (*     match Mem.storev Mptr m1 (Val.offset_ptr sp pos) rs#SP cp with *)
+  (*     | None => Stuck *)
+  (*     | Some m2 => Next (nextinstr (rs #X30 <- (rs SP) #SP <- sp #X31 <- Vundef)) m2 *)
+  (*     end *)
+  (* | Pfreeframe sz pos => *)
+  (*     match Mem.loadv Mptr m (Val.offset_ptr rs#SP pos) (Some cp) with *)
+  (*     | None => Stuck *)
+  (*     | Some v => *)
+  (*         match rs SP with *)
+  (*         | Vptr stk ofs => *)
+  (*             match Mem.free m stk 0 sz cp with *)
+  (*             | None => Stuck *)
+  (*             | Some m' => Next (nextinstr (rs#SP <- v #X31 <- Vundef)) m' *)
+  (*             end *)
+  (*         | _ => Stuck *)
+  (*         end *)
+  (*     end *)
   | Plabel lbl =>
-      Next (nextinstr rs) m
-  | Ploadsymbol rd s ofs =>
-      Next (nextinstr (rs#rd <- (Genv.symbol_address ge s ofs))) m
-  | Ploadsymbol_high rd s ofs =>
-      Next (nextinstr (rs#rd <- (high_half ge s ofs))) m
+      (nextinstr rs) m
+  | Pptrbr r lbl1 lbl2 =>
+      eval_ptr_branch f lbl1 lbl2 rs m (rs##r)
+  (* | Ploadsymbol rd s ofs => *)
+  (*      (nextinstr (rs#rd <- (Genv.symbol_address ge s ofs))) m *)
+  (* | Ploadsymbol_high rd s ofs => *)
+  (*      (nextinstr (rs#rd <- (high_half ge s ofs))) m *)
   | Ploadli rd i =>
-      Next (nextinstr (rs#X31 <- Vundef #rd <- (Vlong i))) m
+       (nextinstr (rs#X31 <- OCVundef #rd <- (OCVlong i))) m
   | Ploadfi rd f =>
-      Next (nextinstr (rs#X31 <- Vundef #rd <- (Vfloat f))) m
+       (nextinstr (rs#X31 <- OCVundef #rd <- (OCVfloat f))) m
   | Ploadsi rd f =>
-      Next (nextinstr (rs#X31 <- Vundef #rd <- (Vsingle f))) m
+       (nextinstr (rs#X31 <- OCVundef #rd <- (OCVsingle f))) m
   | Pbtbl r tbl =>
       match rs r with
-      | Vint n =>
+      | OCVint n =>
           match list_nth_z tbl (Int.unsigned n) with
           | None => Stuck
-          | Some lbl => goto_label f lbl (rs#X5 <- Vundef #X31 <- Vundef) m
+          | Some lbl => goto_label f lbl (rs#X5 <- OCVundef #X31 <- OCVundef) m
           end
       | _ => Stuck
       end
   | Pbuiltin ef args res =>
       Stuck (**r treated specially below *)
+  | Pfail => Crashed
 
   (** The following instructions and directives are not generated directly by Asmgen,
       so we do not model them. *)
+  | PCloadtag _ _ (* TODO /!\  -- needed by Asmgen *)
   | Pfence
 
   | Pfmvxs _ _
@@ -1163,7 +1644,7 @@ Definition exec_instr (f: function) (i: instruction) (rs: regset) (m: mem) (cp: 
 (*   end. *)
 
 (** Translation of the LTL/Linear/Mach view of machine registers to
-  the RISC-V view.  Note that no LTL register maps to [X31].  This
+  the RISC-V view.  Note that no LTL register maps to [X31 X32].  This
   register is reserved as temporary, to be used by the generated RV32G
   code.  *)
 
@@ -1191,25 +1672,24 @@ Definition preg_of (r: mreg) : preg :=
 
 Definition undef_caller_save_regs (rs: regset) : regset :=
   fun r =>
-    if preg_eq r SP
+    if preg_eq r SPC
     || In_dec preg_eq r (List.map preg_of (List.filter is_callee_save all_mregs))
     then rs r
-    else Vundef.
+    else OCVundef.
 
 (** Extract the values of the arguments of an external call.
     We exploit the calling conventions from module [Conventions], except that
     we use RISC-V registers instead of locations. *)
 
-Inductive extcall_arg (rs: regset) (m: mem): loc -> val -> Prop :=
+Inductive extcall_arg (rs: regset) (m: mem): caploc -> ocval -> Prop :=
   | extcall_arg_reg: forall r,
       extcall_arg rs m (R r) (rs (preg_of r))
   | extcall_arg_stack: forall ofs ty bofs cp v,
       bofs = Stacklayout.fe_ofs_arg + 4 * ofs ->
-      Mem.loadv (chunk_of_type ty) m
-                (Val.offset_ptr rs#SP (Ptrofs.repr bofs)) cp = Some v ->
+      Mem.loadv UNINIT (chunk_of_type ty) m rs#SPC (OCVstackptr bofs) cp false = inl v ->
       extcall_arg rs m (S Outgoing ofs ty) v.
 
-Inductive extcall_arg_pair (rs: regset) (m: mem): rpair loc -> val -> Prop :=
+Inductive extcall_arg_pair (rs: regset) (m: mem): rpair caploc -> ocval -> Prop :=
   | extcall_arg_one: forall l v,
       extcall_arg rs m l v ->
       extcall_arg_pair rs m (One l) v
@@ -1219,67 +1699,67 @@ Inductive extcall_arg_pair (rs: regset) (m: mem): rpair loc -> val -> Prop :=
       extcall_arg_pair rs m (Twolong hi lo) (Val.longofwords vhi vlo).
 
 Definition extcall_arguments
-    (rs: regset) (m: mem) (sg: signature) (args: list val) : Prop :=
-  list_forall2 (extcall_arg_pair rs m) (loc_arguments sg) args.
+    (rs: regset) (m: mem) (sg: capsignature) (args: list ocval) : Prop :=
+  list_forall2 (extcall_arg_pair rs m) (caploc_arguments sg) args.
 
-Definition loc_external_result (sg: signature) : rpair preg :=
-  map_rpair preg_of (loc_result sg).
+Definition loc_external_result (sg: capsignature) : rpair preg :=
+  map_rpair preg_of (caploc_result sg).
 
 (** Execution of the instruction at [rs PC]. *)
 
-Inductive stackframe: Type :=
-| Stackframe:
-    forall (f: block)       (**r pointer to calling function *)
-      (sp: val)         (**r stack pointer in calling function *)
-      (retaddr: ptrofs), (**r Asm return address in calling function *)
-      stackframe.
+(* Inductive stackframe: Type := *)
+(* | Stackframe: *)
+(*     forall (f: block)       (**r pointer to calling function *) *)
+(*       (sp: val)         (**r stack pointer in calling function *) *)
+(*       (retaddr: ptrofs), (**r Asm return address in calling function *) *)
+(*       stackframe. *)
 
-Definition stack := list stackframe.
+(* Definition stack := list stackframe. *)
 
-(* The state of the stack when we start the execution *)
-Definition initial_stack: stack := nil.
+(* (* The state of the stack when we start the execution *) *)
+(* Definition initial_stack: stack := nil. *)
 
-(* Updates to the stack *)
-(* These two definitions shouldn't really do any real enforcement. Instead,
-   they should just be used to keep track of the stack and use it in the
-   invariants *)
-(* The two definitions only update the stack when a cross-compartment change
-   is detected *)
-Definition update_stack_call (s: stack) (cp: compartment) rs' :=
-  let pc' := rs' # PC in
-  let ra' := rs' # RA in
-  let sp' := rs' # SP in
-  (* match Genv.find_comp ge pc' with *)
-  (* | Some cp' => *)
-  if Pos.eqb cp (Genv.find_comp ge pc') then
-    (* If we are in the same compartment as previously recorded, we
-         don't update the stack *)
-    Some s
-  else
-    (* Otherwise, we simply push a new frame on the stack *)
-    match ra' with
-    | Vptr f retaddr =>
-        Some (Stackframe f sp' retaddr :: s)
-    | _ => None
-    end
-  .
+(* (* Updates to the stack *) *)
+(* (* These two definitions shouldn't really do any real enforcement. Instead, *)
+(*    they should just be used to keep track of the stack and use it in the *)
+(*    invariants *) *)
+(* (* The two definitions only update the stack when a cross-compartment change *)
+(*    is detected *) *)
+(* Definition update_stack_call (s: stack) (cp: compartment) rs' := *)
+(*   let pc' := rs' # PC in *)
+(*   let ra' := rs' # RA in *)
+(*   let sp' := rs' # SP in *)
+(*   (* match Genv.find_comp ge pc' with *) *)
+(*   (* | Some cp' => *) *)
+(*   if Pos.eqb cp (Genv.find_comp ge pc') then *)
+(*     (* If we are in the same compartment as previously recorded, we *)
+(*          don't update the stack *) *)
+(*     Some s *)
+(*   else *)
+(*     (* Otherwise, we simply push a new frame on the stack *) *)
+(*     match ra' with *)
+(*     | Vptr f retaddr => *)
+(*         Some (Stackframe f sp' retaddr :: s) *)
+(*     | _ => None *)
+(*     end *)
+(*   . *)
 
-Definition update_stack_return (s: stack) (cp: compartment) rs' :=
-  let pc' := rs' # PC in
-  if Pos.eqb cp (Genv.find_comp ge pc') then
-    (* If we are in the same compartment as previously recorded, we
-         don't update the stack *)
-    Some s
-  else
-    (* Otherwise we just pop the top stackframe, if it exists *)
-    match s with
-    | nil => Some nil
-    | _ :: st' => Some st'
-    end
-  .
+(* Definition update_stack_return (s: stack) (cp: compartment) rs' := *)
+(*   let pc' := rs' # PC in *)
+(*   if Pos.eqb cp (Genv.find_comp ge pc') then *)
+(*     (* If we are in the same compartment as previously recorded, we *)
+(*          don't update the stack *) *)
+(*     Some s *)
+(*   else *)
+(*     (* Otherwise we just pop the top stackframe, if it exists *) *)
+(*     match s with *)
+(*     | nil => Some nil *)
+(*     | _ :: st' => Some st' *)
+(*     end *)
+(*   . *)
 
 Inductive state: Type :=
-  | State: stack -> regset -> mem -> state.
+  | State: regset -> mem -> state.
 
 (* Definition is_call i := *)
 (*   match i with *)
@@ -1287,237 +1767,277 @@ Inductive state: Type :=
 (*   | _ => false *)
 (*   end. *)
 
+(* ALG: a call is denoted by a capability jump and link, which seals the next instruction in RA *)
 Definition sig_call i :=
   match i with
-  | Pjal_s _ sig flag | Pjal_r _ sig flag =>
-                          if flag then Some sig else None
+  | PCjal_r _ _ sig flag =>
+      if flag then Some sig else None
   | _ => None
   end.
 
 (* Probably need to do the same thing and to define a [sig_return] function *)
-Definition is_return i :=
+(* ALG: a return is denotes by a sealed invocation *)
+Definition is_return i rs :=
   match i with
-  | Pj_r _ _ flag => flag
+  | PCinvoke _ r_data flag =>
+      match rs###r_data with
+      | OCVcap (OCsealed _ (OCVmem _ Directed _ _ _)) => flag
+      | _ => false
+      end
   | _ => false
   end.
 
-Definition asm_parent_ra s :=
-  match s with
-  | nil => Vnullptr
-  | Stackframe b sp retaddr :: _ => Vptr b retaddr
-  end.
+(* Definition asm_parent_ra s := *)
+(*   match s with *)
+(*   | nil => Vnullptr *)
+(*   | Stackframe b sp retaddr :: _ => Vptr b retaddr *)
+(*   end. *)
 
-Definition asm_parent_sp s :=
-  match s with
-  | nil => Vnullptr
-  | Stackframe b sp retaddr :: _ => sp
-  end.
+(* Definition asm_parent_sp s := *)
+(*   match s with *)
+(*   | nil => Vnullptr *)
+(*   | Stackframe b sp retaddr :: _ => sp *)
+(*   end. *)
 
 Inductive step: state -> trace -> state -> Prop :=
   | exec_step_internal:
-      forall b ofs f i rs m rs' m' b' ofs' st cp,
-      rs PC = Vptr b ofs ->
-      Genv.find_funct_ptr ge b = Some (Internal f) ->
-      find_instr (Ptrofs.unsigned ofs) (fn_code f) = Some i ->
-      forall (COMP: Genv.find_comp ge (rs PC) = cp),
+    forall c ofs f i rs m rs' m' c' cp,
+      get_addr c = ofs ->
+      executeAllowedCap c = true -> (* checks that the program counter is unsealed and has executable permission *)
+      rs PCC = OCVcap c ->
+      Genv.find_funct_ptr ge c = Some (Internal f) ->
+      find_instr (Ptrofs.unsigned ofs) (fn_wrapper f ++ fn_code f) = Some i ->
+      forall (COMP: Genv.find_comp ge (rs PCC) = cp),
       exec_instr f i rs m cp = Next rs' m' ->
       sig_call i = None ->
-      is_return i = false ->
-      forall (NEXTPC: rs' PC = Vptr b' ofs'),
-      forall (ALLOWED: Genv.allowed_call ge (comp_of f) (Vptr b' ofs')),
-      step (State st rs m) E0 (State st rs' m')
+      is_return i rs = false ->
+      forall (NEXTPC: rs' PCC = OCVcap c'),
+      (* forall (ALLOWED: Genv.allowed_call ge (comp_of f) (Vptr b' ofs')), *) (* ownership of the capability determines allowed calls *)
+      step (State rs m) E0 (State rs' m')
   | exec_step_internal_call:
-      forall b ofs f i sig rs m rs' m' b' ofs' cp st st',
-      rs PC = Vptr b ofs ->
-      Genv.find_funct_ptr ge b = Some (Internal f) ->
-      find_instr (Ptrofs.unsigned ofs) (fn_code f) = Some i ->
+      forall c ofs f i sig rs m rs' m' c' cp,
+      get_addr c = ofs ->
+      executeAllowedCap c = true -> (* checks that the program counter is unsealed and has executable permission *)
+      rs PCC = OCVcap c ->
+      Genv.find_funct_ptr ge c = Some (Internal f) ->
+      find_instr (Ptrofs.unsigned ofs) (fn_wrapper f ++ fn_code f) = Some i ->
       exec_instr f i rs m cp = Next rs' m' ->
       sig_call i = Some sig ->
-      forall (NEXTPC: rs' PC = Vptr b' ofs'),
-      forall (ALLOWED: Genv.allowed_call ge (comp_of f) (Vptr b' ofs')),
-      forall (CURCOMP: Genv.find_comp ge (Vptr b Ptrofs.zero) = cp),
+      forall (NEXTPC: rs' PCC = OCVcap c'),
+      (* forall (ALLOWED: Genv.allowed_call ge (comp_of f) (Vptr b' ofs')), *) (* ownership of the capability determines allowed calls *)
+      forall (ALLOWED: Genv.allowed_call_capability ge (OCVcap c')), (* a step is only flagged as a call if it targets an E capability of the environment *)
+      forall (CURCOMP: Genv.find_comp ge (OCVcap c) = cp),
       (* Is a call, we update the stack *)
-      forall (STUPD: update_stack_call st cp rs' = Some st'),
+      (* forall (STUPD: update_stack_call st cp rs' = Some st'), *)
+        
       (* Is a call, we check whether we are allowed to pass pointers *)
-      forall (NO_CROSS_PTR_REGS:
-          Genv.type_of_call ge (comp_of f) (Genv.find_comp ge (Vptr b' ofs')) = Genv.CrossCompartmentCall ->
-          forall r, List.In (R r) (regs_of_rpairs (loc_parameters sig)) ->
-               not_ptr (rs' (preg_of r))),
-      forall (NO_CROSS_PTR_STACK:
-          Genv.type_of_call ge (comp_of f) (Genv.find_comp ge (Vptr b' ofs')) = Genv.CrossCompartmentCall ->
-          forall ofs v ty,
-            List.In (S Incoming ofs ty) (regs_of_rpairs (loc_parameters sig)) ->
-            Mem.loadv (chunk_of_type ty) m
-              (Val.offset_ptr (rs' SP) (* this is the stack pointer *)
-                 (Ptrofs.repr (offset_arg ofs))) None
-                      = Some v ->
-            (* load_stack m sp ty (Ptrofs.repr (offset_arg ofs)) None = Some v -> *)
-            not_ptr v),
-      step (State st rs m) E0 (State st' rs' m')
+      (* forall (NO_CROSS_PTR_REGS: *)
+      (*     Genv.type_of_call ge (comp_of f) (Genv.find_comp ge (OCVcap c')) = Genv.CrossCompartmentCall -> *)
+      (*     forall r, List.In (R r) (regs_of_rpairs (caploc_parameters sig)) -> *)
+      (*          not_ptr (rs' (preg_of r))), *)
+      (* forall (NO_CROSS_PTR_STACK: *)
+      (*     Genv.type_of_call ge (comp_of f) (Genv.find_comp ge (Vptr b' ofs')) = Genv.CrossCompartmentCall -> *)
+      (*     forall ofs v ty, *)
+      (*       List.In (S Incoming ofs ty) (regs_of_rpairs (loc_parameters sig)) -> *)
+      (*       Mem.loadv (chunk_of_type ty) m *)
+      (*         (Val.offset_ptr (rs' SP) (* this is the stack pointer *) *)
+      (*            (Ptrofs.repr (offset_arg ofs))) None *)
+      (*                 = Some v -> *)
+      (*       (* load_stack m sp ty (Ptrofs.repr (offset_arg ofs)) None = Some v -> *) *)
+      (*       not_ptr v), *)
+      (* The capability secure calling convention enforces the above:
+      all functions are surrounded by wrappers that zero out
+      registers, and checks that parameters are well typed. moreover,
+      the calling convention makes sure not to pass any faulty stack
+      pointers *)
+        
+      step (State rs m) E0 (State rs' m')
   | exec_step_internal_return:
-      forall b ofs f i rs m rs' m' cp cp' st st',
-      rs PC = Vptr b ofs ->
-      Genv.find_funct_ptr ge b = Some (Internal f) ->
-      find_instr (Ptrofs.unsigned ofs) (fn_code f) = Some i ->
+      forall c ofs f i rs m rs' m' cp cp',
+      get_addr c = ofs ->
+      executeAllowedCap c = true ->
+      rs PCC = OCVcap c ->
+      Genv.find_funct_ptr ge c = Some (Internal f) ->
+      find_instr (Ptrofs.unsigned ofs) (fn_wrapper f ++ fn_code f) = Some i ->
       exec_instr f i rs m cp = Next rs' m' ->
-      is_return i = true ->
-      forall (CURCOMP: Genv.find_comp ge (rs PC) = cp),
-      forall (NEXTCOMP: Genv.find_comp ge (rs' PC) = cp'),
+      is_return i rs = true ->
+      forall (CURCOMP: Genv.find_comp ge (rs PCC) = cp),
+      forall (NEXTCOMP: Genv.find_comp ge (rs' PCC) = cp'),
+
       (* We only impose conditions on when returns can be executed for cross-compartment
          returns. These conditions are that we restore the previous RA and SP *)
-      forall (PC_RA: cp <> cp' -> rs' PC = asm_parent_ra st),
-      forall (RESTORE_SP: cp <> cp' -> rs' SP = asm_parent_sp st),
+      (* forall (PC_RA: cp <> cp' -> rs' PCC = asm_parent_ra st), *)
+      (* forall (RESTORE_SP: cp <> cp' -> rs' SP = asm_parent_sp st), *)
       (* Note that in the same manner, this definition only updates the stack when doing
          cross-compartment returns *)
-      forall (STUPD: update_stack_return st cp rs' = Some st'),
+      (* forall (STUPD: update_stack_return st cp rs' = Some st'), *)
+
       (* (* No cross-compartment pointer return *) *)
-      forall (NO_CROSS_PTR:
-          Genv.type_of_call ge cp' cp = Genv.CrossCompartmentCall ->
-          forall r, List.In r (regs_of_rpair (loc_result (fn_sig f))) ->
-              not_ptr (rs' (preg_of r))),
-      step (State st rs m) E0 (State st' rs' m')
+      (* forall (NO_CROSS_PTR: *)
+      (*     Genv.type_of_call ge cp' cp = Genv.CrossCompartmentCall -> *)
+      (*     forall r, List.In r (regs_of_rpair (loc_result (fn_sig f))) -> *)
+      (*          not_ptr (rs' (preg_of r))), *)
+      (* For the above to hold, it is up to the caller to do this check. TODO: discuss! *)  
+        
+      step (State rs m) E0 (State rs' m')
   | exec_step_builtin:
-      forall b ofs f ef args res rs m vargs t vres rs' m' st,
-      rs PC = Vptr b ofs ->
-      Genv.find_funct_ptr ge b = Some (Internal f) ->
-      find_instr (Ptrofs.unsigned ofs) f.(fn_code) = Some (Pbuiltin ef args res) ->
-      eval_builtin_args ge rs (rs SP) m args vargs ->
-      external_call ef ge (comp_of f) vargs m t vres m' ->
-      rs' = nextinstr
-              (set_res res vres
-                (undef_regs (map preg_of (destroyed_by_builtin ef))
-                   (rs#X31 <- Vundef))) ->
-      step (State st rs m) t (State st rs' m')
+      forall c ofs f ef args res rs m (* vargs *) t vres (rs' : regset) m',
+      get_addr c = ofs ->
+      executeAllowedCap c = true ->
+      rs PCC = OCVcap c ->
+      Genv.find_funct_ptr ge c = Some (Internal f) ->
+      find_instr (Ptrofs.unsigned ofs) (fn_wrapper f ++ fn_code f) = Some (Pbuiltin ef args res) ->
+      (* eval_builtin_args ge rs (rs SPC) m args vargs -> *)
+      (* external_call ef ge (comp_of f) vargs m t vres m' ->  *)
+  (* TODO: external calls are currently parametrized by the common environment *)
+  (* definition, maybe use some kind of subtyping? or redo all definitions.... *)
+      nextinstr
+        (set_res res vres
+                 (undef_regs (map preg_of (destroyed_by_builtin ef))
+                             (rs#X31 <- OCVundef))) m = Next rs' m' ->
+      step (State rs m) t (State rs' m')
   | exec_step_external:
-      forall b ef args res rs m t rs' m' cp cp' cp'' st st',
-      rs PC = Vptr b Ptrofs.zero ->
-      Genv.find_funct_ptr ge b = Some (External ef) ->
-      forall COMP: Genv.find_comp ge (rs RA) = cp,
-      external_call ef ge cp args m t res m' ->
-      extcall_arguments rs m (ef_sig ef) args ->
-      rs' = (set_pair (loc_external_result (ef_sig ef) ) res (undef_caller_save_regs rs))#PC <- (rs RA) ->
+      forall c ef (* args res  *)rs m t rs' m' cp cp' cp'',
+      get_addr c = get_lo c ->
+      executeAllowedCap c = true ->
+      rs PCC = OCVcap c ->
+      Genv.find_funct_ptr ge c = Some (External ef) ->
+      forall COMP: Genv.find_comp ge (rs RAC) = cp,
+
+      (* external_call ef ge cp args m t res m' -> *) (* TODO: same as above *)
+      (* extcall_arguments rs m (ef_sig ef) args -> *) (* TODO *)
+      (* rs' = (set_pair (loc_external_result (ef_sig ef) ) res (undef_caller_save_regs rs))#PCC <- (rs RAC) -> *) (* TODO: same as above. something is off with how i do define the new more detailed environment *)
+
       (* These steps behave like returns. So we must update the stack *)
-      forall (CURCOMP: Genv.find_comp ge (rs PC) = cp'),
-      forall (NEXTCOMP: Genv.find_comp ge (rs' PC) = cp''),
+      forall (CURCOMP: Genv.find_comp ge (rs PCC) = cp'),
+      forall (NEXTCOMP: Genv.find_comp ge (rs' PCC) = cp''),
       (* We only impose conditions on when returns can be executed for cross-compartment
          returns. These conditions are that we restore the previous RA and SP *)
-      forall (PC_RA: cp' <> cp'' -> rs' PC = asm_parent_ra st),
-      forall (RESTORE_SP: cp' <> cp'' -> rs' SP = asm_parent_sp st),
+      (* forall (PC_RA: cp' <> cp'' -> rs' PCC = asm_parent_ra st), *)
+      (* forall (RESTORE_SP: cp' <> cp'' -> rs' SPC = asm_parent_sp st), *)
       (* Note that in the same manner, this definition only updates the stack when doing
          cross-compartment returns *)
-      forall (STUPD: update_stack_return st cp' rs' = Some st'),
-      step (State st rs m) t (State st' rs' m').
+      step (State rs m) t (State rs' m').
 
 End RELSEM.
 
 (** Execution of whole programs. *)
 
-Inductive initial_state (p: program): state -> Prop :=
-  | initial_state_intro: forall m0,
-      let ge := Genv.globalenv p in
+Parameter stack_size: Z.
+Parameter heap_size: Z.
+Parameter seal_size: compartment -> program -> Z. (* TODO: define this one here? *)
+Parameter seal_size_pos: forall c gls, seal_size c gls >= 0.
+
+Definition globalenv := Genv.globalenv stack_size heap_size seal_size seal_size_pos.
+Definition init_mem := Genv.init_mem stack_size heap_size seal_size seal_size_pos.
+
+Inductive initial_state (p: program) (gstart gend sstart send : ptrofs) : state -> Prop :=
+  | initial_state_intro: forall m0 ge,
+      globalenv p gstart gend sstart send = Some ge ->
       let rs0 :=
-        (Pregmap.init Vundef)
-        # PC <- (Genv.symbol_address ge p.(prog_main) Ptrofs.zero)
-        # SP <- Vnullptr
-        # RA <- Vnullptr in
-      Genv.init_mem p = Some m0 ->
-      initial_state p (State initial_stack rs0 m0).
+        (Pregmap.init OCVundef)
+        # PCC <- (Genv.symbol_address ge p.(prog_main) Ptrofs.zero)
+        # SPC <- OCVnullcap
+                  # RAC <- Vnullptr in
+      init_mem p gstart gend sstart send = Some m0 ->
+      initial_state p gstart gend sstart send (State rs0 m0).
 
 Inductive final_state: state -> int -> Prop :=
   | final_state_intro: forall rs m r,
-      rs PC = Vnullptr ->
-      rs X10 = Vint r ->
-      final_state (State initial_stack rs m) r.
+      rs PCC = Vnullptr ->
+      rs X10 = OCVint r ->
+      final_state (State rs m) r.
 
-Definition semantics (p: program) :=
-  Semantics step (initial_state p) final_state (Genv.globalenv p).
+Definition semantics (p: program) (gstart gend sstart send : ptrofs) :=
+  do X <- (globalenv p gstart gend sstart send);
+  Some (Semantics_alt Genv.to_senv step (initial_state p gstart gend sstart send) final_state X).
 
 (** Determinacy of the [Asm] semantics. *)
 
-Remark extcall_arguments_determ:
-  forall rs m sg args1 args2,
-  extcall_arguments rs m sg args1 -> extcall_arguments rs m sg args2 -> args1 = args2.
-Proof.
-  intros until m.
-  assert (A: forall l v1 v2,
-             extcall_arg rs m l v1 -> extcall_arg rs m l v2 -> v1 = v2).
-  { intros. inv H; inv H0. congruence.
-    destruct (rs X2); try discriminate.
-    simpl in H2, H5.
-    apply Mem.load_result in H2.
-    apply Mem.load_result in H5. congruence. }
-  assert (B: forall p v1 v2,
-             extcall_arg_pair rs m p v1 -> extcall_arg_pair rs m p v2 -> v1 = v2).
-  { intros. inv H; inv H0. 
-    eapply A; eauto.
-    f_equal; eapply A; eauto. }
-  assert (C: forall ll vl1, list_forall2 (extcall_arg_pair rs m) ll vl1 ->
-             forall vl2, list_forall2 (extcall_arg_pair rs m) ll vl2 -> vl1 = vl2).
-  {
-    induction 1; intros vl2 EA; inv EA.
-    auto.
-    f_equal; eauto. }
-  intros. eapply C; eauto.
-Qed.
+(* Remark extcall_arguments_determ: *)
+(*   forall rs m sg args1 args2, *)
+(*   extcall_arguments rs m sg args1 -> extcall_arguments rs m sg args2 -> args1 = args2. *)
+(* Proof. *)
+(*   intros until m. *)
+(*   assert (A: forall l v1 v2, *)
+(*              extcall_arg rs m l v1 -> extcall_arg rs m l v2 -> v1 = v2). *)
+(*   { intros. inv H; inv H0. congruence. *)
+(*     destruct (rs X2); try discriminate. *)
+(*     simpl in H2, H5. *)
+(*     apply Mem.load_result in H2. *)
+(*     apply Mem.load_result in H5. congruence. } *)
+(*   assert (B: forall p v1 v2, *)
+(*              extcall_arg_pair rs m p v1 -> extcall_arg_pair rs m p v2 -> v1 = v2). *)
+(*   { intros. inv H; inv H0.  *)
+(*     eapply A; eauto. *)
+(*     f_equal; eapply A; eauto. } *)
+(*   assert (C: forall ll vl1, list_forall2 (extcall_arg_pair rs m) ll vl1 -> *)
+(*              forall vl2, list_forall2 (extcall_arg_pair rs m) ll vl2 -> vl1 = vl2). *)
+(*   { *)
+(*     induction 1; intros vl2 EA; inv EA. *)
+(*     auto. *)
+(*     f_equal; eauto. } *)
+(*   intros. eapply C; eauto. *)
+(* Qed. *)
 
-(* RB: NOTE: In the next proof, the wrapped [exec_instr] would require extra
-   processing, such as this. *)
-(* Ltac peel_exec_instr := *)
+(* (* RB: NOTE: In the next proof, the wrapped [exec_instr] would require extra *)
+(*    processing, such as this. *) *)
+(* (* Ltac peel_exec_instr := *) *)
+(* (*   match goal with *) *)
+(* (*   | Hexec : exec_instr _ _ _ ?RS ?M = _, *) *)
+(* (*     Hpc : ?RS PC = Vptr ?B _ |- _ *) *)
+(* (*     => *) *)
+(* (*     unfold exec_instr in Hexec; *) *)
+(* (*     rewrite Hpc in Hexec; *) *)
+(* (*     destruct ((Mem.mem_compartments M) ! B) *) *)
+(* (*   end. *) *)
+
+(* Lemma semantics_determinate: forall p, determinate (semantics p). *)
+(* Proof. *)
+(* Ltac Equalities := *)
 (*   match goal with *)
-(*   | Hexec : exec_instr _ _ _ ?RS ?M = _, *)
-(*     Hpc : ?RS PC = Vptr ?B _ |- _ *)
-(*     => *)
-(*     unfold exec_instr in Hexec; *)
-(*     rewrite Hpc in Hexec; *)
-(*     destruct ((Mem.mem_compartments M) ! B) *)
+(*   | [ H1: ?a = ?b, H2: ?a = ?c |- _ ] => *)
+(*       rewrite H1 in H2; inv H2; Equalities *)
+(*   | _ => idtac *)
 (*   end. *)
+(*   intros; constructor; simpl; intros. *)
+(* - (* determ *) *)
+(*   inv H; inv H0; Equalities; try now discriminate. *)
+(*   + split. constructor. auto. *)
+(*   + split. constructor. auto. *)
+(*   + now destruct i0. *)
+(*   + now destruct i0. *)
+(*   + split. constructor. congruence. *)
 
-Lemma semantics_determinate: forall p, determinate (semantics p).
-Proof.
-Ltac Equalities :=
-  match goal with
-  | [ H1: ?a = ?b, H2: ?a = ?c |- _ ] =>
-      rewrite H1 in H2; inv H2; Equalities
-  | _ => idtac
-  end.
-  intros; constructor; simpl; intros.
-- (* determ *)
-  inv H; inv H0; Equalities; try now discriminate.
-  + split. constructor. auto.
-  + split. constructor. auto.
-  + now destruct i0.
-  + now destruct i0.
-  + split. constructor. congruence.
-
-  + assert (vargs0 = vargs) by (eapply eval_builtin_args_determ; eauto). subst vargs0.
-    exploit external_call_determ. eexact H5. eexact H14.  intros [A B].
-    split. auto. intros. destruct B; auto. subst. auto.
-  + assert (args0 = args) by (eapply extcall_arguments_determ; eauto). subst args0.
-    exploit external_call_determ. eexact H3. eexact H9. intros [A B].
-    split. auto. intros. destruct B; auto. subst. congruence.
-- (* trace length *)
-  red; intros. inv H; simpl.
-  omega.
-  omega.
-  omega.
-  eapply external_call_trace_length; eauto.
-  eapply external_call_trace_length; eauto.
-- (* initial states *)
-  inv H; inv H0. f_equal. congruence.
-- (* final no step *)
-  assert (NOTNULL: forall b ofs, Vnullptr <> Vptr b ofs).
-  { intros; unfold Vnullptr; destruct Archi.ptr64; congruence. }
-  inv H. unfold Vzero in H0. red; intros; red; intros.
-  inv H; rewrite H0 in *; eelim NOTNULL; eauto.
-- (* final states *)
-  inv H; inv H0. congruence.
-Qed.
+(*   + assert (vargs0 = vargs) by (eapply eval_builtin_args_determ; eauto). subst vargs0. *)
+(*     exploit external_call_determ. eexact H5. eexact H14.  intros [A B]. *)
+(*     split. auto. intros. destruct B; auto. subst. auto. *)
+(*   + assert (args0 = args) by (eapply extcall_arguments_determ; eauto). subst args0. *)
+(*     exploit external_call_determ. eexact H3. eexact H9. intros [A B]. *)
+(*     split. auto. intros. destruct B; auto. subst. congruence. *)
+(* - (* trace length *) *)
+(*   red; intros. inv H; simpl. *)
+(*   omega. *)
+(*   omega. *)
+(*   omega. *)
+(*   eapply external_call_trace_length; eauto. *)
+(*   eapply external_call_trace_length; eauto. *)
+(* - (* initial states *) *)
+(*   inv H; inv H0. f_equal. congruence. *)
+(* - (* final no step *) *)
+(*   assert (NOTNULL: forall b ofs, Vnullptr <> Vptr b ofs). *)
+(*   { intros; unfold Vnullptr; destruct Archi.ptr64; congruence. } *)
+(*   inv H. unfold Vzero in H0. red; intros; red; intros. *)
+(*   inv H; rewrite H0 in *; eelim NOTNULL; eauto. *)
+(* - (* final states *) *)
+(*   inv H; inv H0. congruence. *)
+(* Qed. *)
 
 (** Classification functions for processor registers (used in Asmgenproof). *)
 
 Definition data_preg (r: preg) : bool :=
   match r with
-  | IR RA  => false
+  | IR RAC  => false
   | IR X31 => false
   | IR _   => true
   | FR _   => true
